<rdf:RDF
    xmlns:rdf="http://www.w3.org/1999/02/22-rdf-syntax-ns#"
    xmlns:cd="http://www.openmath.org/cd/"
    xmlns:oo="http://omdoc.org/ontology#"
    xmlns:owl="http://www.w3.org/2002/07/owl#"
    xmlns:dct="http://purl.org/dc/terms/"
    xmlns:xsd="http://www.w3.org/2001/XMLSchema#"
    xmlns:omo="http://www.openmath.org/ontology#"
    xmlns:rdfs="http://www.w3.org/2000/01/rdf-schema#" > 
  <rdf:Description rdf:about="http://www.openmath.org/ontology#type">
    <rdf:type rdf:resource="http://www.w3.org/2002/07/owl#ObjectProperty"/>
    <rdf:type rdf:resource="http://www.w3.org/2002/07/owl#InverseFunctionalProperty"/>
    <owl:inverseOf rdf:resource="http://www.openmath.org/ontology#typesSymbol"/>
    <rdfs:isDefinedBy rdf:resource="http://www.openmath.org/ontology#"/>
  </rdf:Description>
  <rdf:Description rdf:about="http://www.openmath.org/ontology#hasDirectPart">
    <rdf:type rdf:resource="http://www.w3.org/2002/07/owl#InverseFunctionalProperty"/>
    <rdf:type rdf:resource="http://www.w3.org/2002/07/owl#ObjectProperty"/>
    <rdfs:subPropertyOf rdf:resource="http://www.openmath.org/ontology#hasPart"/>
    <rdfs:comment>This relation denotes that one concept A directly logically contains another concept B, and that B is not contained by any other concept than A, as reflected by child elements in OpenMath XML documents.</rdfs:comment>
    <rdfs:isDefinedBy rdf:resource="http://www.openmath.org/ontology#"/>
  </rdf:Description>
  <rdf:Description rdf:about="http://purl.org/dc/terms/identifier">
    <rdf:type rdf:resource="http://www.w3.org/2002/07/owl#DatatypeProperty"/>
  </rdf:Description>
  <rdf:Description rdf:nodeID="A0">
    <rdf:type rdf:resource="http://www.w3.org/2002/07/owl#Restriction"/>
    <owl:onProperty rdf:resource="http://www.openmath.org/ontology#role"/>
    <owl:maxCardinality rdf:datatype="http://www.w3.org/2001/XMLSchema#nonNegativeInteger">1</owl:maxCardinality>
  </rdf:Description>
  <rdf:Description rdf:about="http://www.openmath.org/ontology#reviewDate">
    <rdf:type rdf:resource="http://www.w3.org/2002/07/owl#DatatypeProperty"/>
    <rdf:type rdf:resource="http://www.w3.org/2002/07/owl#FunctionalProperty"/>
    <rdfs:domain rdf:resource="http://www.openmath.org/ontology#Dictionary"/>
    <rdfs:range rdf:resource="http://www.w3.org/2001/XMLSchema#date"/>
    <rdfs:comment>The review date of a content dictionary or signature dictionary, as described in section 4.2 and 4.3.2</rdfs:comment>
    <rdfs:isDefinedBy rdf:resource="http://www.openmath.org/ontology#"/>
  </rdf:Description>
  <rdf:Description rdf:about="http://www.openmath.org/ontology#Private">
    <rdf:type rdf:resource="http://www.openmath.org/ontology#Status"/>
    <rdfs:comment>The 'private' status of a CD, as described in section 4.2.1</rdfs:comment>
    <rdfs:isDefinedBy rdf:resource="http://www.openmath.org/ontology#"/>
  </rdf:Description>
  <rdf:Description rdf:nodeID="A1">
    <owl:unionOf rdf:nodeID="A2"/>
  </rdf:Description>
  <rdf:Description rdf:about="http://www.openmath.org/ontology#hasCommentedPart">
    <rdf:type rdf:resource="http://www.w3.org/2002/07/owl#ObjectProperty"/>
    <rdf:type rdf:resource="http://www.w3.org/2002/07/owl#FunctionalProperty"/>
    <rdfs:subPropertyOf rdf:resource="http://www.openmath.org/ontology#hasDirectPart"/>
    <rdfs:domain rdf:resource="http://www.openmath.org/ontology#Property"/>
    <rdfs:range rdf:resource="http://www.openmath.org/ontology#CommentedPart"/>
    <rdfs:comment>The relationship of a property container to its commented part (CMP).</rdfs:comment>
    <rdfs:isDefinedBy rdf:resource="http://www.openmath.org/ontology#"/>
  </rdf:Description>
  <rdf:Description rdf:about="http://www.openmath.org/ontology#">
    <rdf:type rdf:resource="http://www.w3.org/2002/07/owl#Ontology"/>
    <dct:title>OpenMath 2.0/3.0 content dictionary ontology</dct:title>
    <rdfs:comment>OpenMath 2.0/3.0 content dictionary ontology in OWL-DL, modeled after the OpenMath 2.0 specification and currently in transition towards OpenMath 3.0.  All references to chapters and sections point to the OpenMath 2.0 standard.</rdfs:comment>
    <dct:creator>Christoph Lange &lt;ch.lange@jacobs-university.de&gt;</dct:creator>
    <dct:subject>Semantic Mathematical Markup</dct:subject>
    <owl:versionInfo>0.3.1</owl:versionInfo>
    <owl:imports rdf:resource="http://omdoc.org/ontology#"/>
  </rdf:Description>
  <rdf:Description rdf:nodeID="A3">
    <rdf:first rdf:resource="http://www.openmath.org/ontology#Error"/>
    <rdf:rest rdf:nodeID="A4"/>
  </rdf:Description>
  <rdf:Description rdf:nodeID="A5">
    <rdf:first rdf:resource="http://www.openmath.org/ontology#Example"/>
    <rdf:rest rdf:resource="http://www.w3.org/1999/02/22-rdf-syntax-ns#nil"/>
  </rdf:Description>
  <rdf:Description rdf:about="http://www.openmath.org/ontology#OpenMathConcept">
    <rdf:type rdf:resource="http://www.w3.org/2002/07/owl#Class"/>
    <rdfs:subClassOf rdf:resource="http://omdoc.org/ontology#MathKnowledgeItem"/>
    <rdfs:comment>The generic superclass of all concepts that can be expressed in OpenMath content/signature/notation dictionaries</rdfs:comment>
    <rdfs:isDefinedBy rdf:resource="http://www.openmath.org/ontology#"/>
  </rdf:Description>
  <rdf:Description rdf:about="http://www.openmath.org/ontology#SemanticAttribution">
    <rdf:type rdf:resource="http://www.openmath.org/ontology#Role"/>
    <rdfs:comment>The 'semantic attribution' role of a symbol, as described in section 2.1.4</rdfs:comment>
    <rdfs:isDefinedBy rdf:resource="http://www.openmath.org/ontology#"/>
  </rdf:Description>
  <rdf:Description rdf:about="http://www.openmath.org/ontology#NotationDefinition">
    <rdf:type rdf:resource="http://www.w3.org/2002/07/owl#Class"/>
    <owl:disjointWith rdf:resource="http://www.openmath.org/ontology#FormalPart"/>
    <owl:disjointWith rdf:resource="http://www.openmath.org/ontology#Role"/>
    <owl:disjointWith rdf:resource="http://www.openmath.org/ontology#Signature"/>
    <owl:disjointWith rdf:resource="http://www.openmath.org/ontology#Status"/>
    <owl:disjointWith rdf:resource="http://www.openmath.org/ontology#CommentedPart"/>
    <owl:disjointWith rdf:resource="http://www.openmath.org/ontology#Example"/>
    <rdfs:isDefinedBy rdf:resource="http://www.openmath.org/ontology#"/>
    <owl:disjointWith rdf:resource="http://www.openmath.org/ontology#CDBase"/>
    <rdfs:subClassOf rdf:resource="http://www.openmath.org/ontology#OpenMathConcept"/>
    <rdfs:comment>A notation definition for one symbol</rdfs:comment>
    <owl:disjointWith rdf:resource="http://www.openmath.org/ontology#Composite"/>
  </rdf:Description>
  <rdf:Description rdf:nodeID="A6">
    <owl:unionOf rdf:nodeID="A7"/>
  </rdf:Description>
  <rdf:Description rdf:about="http://www.openmath.org/ontology#Obsolete">
    <rdf:type rdf:resource="http://www.openmath.org/ontology#Status"/>
    <rdfs:comment>The 'obsolete' status of a CD, as described in section 4.2.1</rdfs:comment>
    <rdfs:isDefinedBy rdf:resource="http://www.openmath.org/ontology#"/>
  </rdf:Description>
  <rdf:Description rdf:about="http://www.openmath.org/ontology#comprises">
    <rdf:type rdf:resource="http://www.w3.org/2002/07/owl#ObjectProperty"/>
    <rdf:type rdf:resource="http://www.w3.org/2002/07/owl#TransitiveProperty"/>
    <rdfs:domain rdf:resource="http://www.openmath.org/ontology#Composite"/>
    <rdfs:range rdf:resource="http://www.openmath.org/ontology#OpenMathConcept"/>
    <rdfs:comment>This relation denotes that one concept A directly or indirectly comprises another concept B, but does not necessarily exclusively contain it.</rdfs:comment>
    <rdfs:isDefinedBy rdf:resource="http://www.openmath.org/ontology#"/>
  </rdf:Description>
  <rdf:Description rdf:about="http://www.openmath.org/ontology#hasNotationDictionary">
    <rdf:type rdf:resource="http://www.w3.org/2002/07/owl#ObjectProperty"/>
    <rdf:type rdf:resource="http://www.w3.org/2002/07/owl#InverseFunctionalProperty"/>
    <owl:inverseOf rdf:resource="http://www.openmath.org/ontology#containsNotationsFor"/>
    <rdfs:isDefinedBy rdf:resource="http://www.openmath.org/ontology#"/>
  </rdf:Description>
  <rdf:Description rdf:nodeID="A8">
    <rdf:first rdf:resource="http://www.openmath.org/ontology#Obsolete"/>
    <rdf:rest rdf:resource="http://www.w3.org/1999/02/22-rdf-syntax-ns#nil"/>
  </rdf:Description>
  <rdf:Description rdf:about="http://www.openmath.org/ontology#Experimental">
    <rdf:type rdf:resource="http://www.openmath.org/ontology#Status"/>
    <rdfs:comment>The 'experimental' status of a CD, as described in section 4.2.1</rdfs:comment>
    <rdfs:isDefinedBy rdf:resource="http://www.openmath.org/ontology#"/>
  </rdf:Description>
  <rdf:Description rdf:about="http://www.openmath.org/ontology#typeSystem">
    <rdf:type rdf:resource="http://www.w3.org/2002/07/owl#ObjectProperty"/>
    <rdf:type rdf:resource="http://www.w3.org/2002/07/owl#FunctionalProperty"/>
    <rdfs:domain rdf:resource="http://www.openmath.org/ontology#SignatureDictionary"/>
    <rdfs:range rdf:nodeID="A1"/>
    <rdfs:comment>The content dictionary [group] that serves as a type system for this signature dictionary, as specified in section 4.4.1.1</rdfs:comment>
    <rdfs:isDefinedBy rdf:resource="http://www.openmath.org/ontology#"/>
  </rdf:Description>
  <rdf:Description rdf:about="http://www.openmath.org/ontology#SymbolDefinition">
    <owl:disjointWith rdf:resource="http://www.openmath.org/ontology#ContentDictionaryGroup"/>
    <rdfs:subClassOf rdf:nodeID="A9"/>
    <rdfs:subClassOf rdf:resource="http://www.openmath.org/ontology#Composite"/>
    <rdfs:comment>An OpenMath symbol definition, as described in section 4.2SD and 4.3.  Some of the properties of symbols are defined as properties in this ontology, others are taken from Dublin Core and RDFS, with the following mapping: Name = dct:identifier, Title = dct:title, CDComment = rdfs:comment.</rdfs:comment>
    <rdfs:comment>OpenMath 3 transitional aspects: Title = dct:title</rdfs:comment>
    <rdf:type rdf:resource="http://www.w3.org/2002/07/owl#Class"/>
    <rdfs:subClassOf rdf:nodeID="A10"/>
    <owl:disjointWith rdf:resource="http://www.openmath.org/ontology#Dictionary"/>
    <rdfs:subClassOf rdf:nodeID="A11"/>
    <rdfs:isDefinedBy rdf:resource="http://www.openmath.org/ontology#"/>
  </rdf:Description>
  <rdf:Description rdf:about="http://purl.org/dc/terms/creator">
    <rdf:type rdf:resource="http://www.w3.org/2002/07/owl#AnnotationProperty"/>
  </rdf:Description>
  <rdf:Description rdf:about="http://www.openmath.org/ontology#usesSymbol">
    <rdf:type rdf:resource="http://www.w3.org/2002/07/owl#ObjectProperty"/>
    <rdfs:domain rdf:nodeID="A12"/>
    <rdfs:range rdf:resource="http://www.openmath.org/ontology#SymbolDefinition"/>
    <rdfs:comment>The relationship of some element to a symbol used in an OpenMath object inside the element</rdfs:comment>
    <rdfs:isDefinedBy rdf:resource="http://www.openmath.org/ontology#"/>
  </rdf:Description>
  <rdf:Description rdf:about="http://www.openmath.org/ontology#Dictionary">
    <rdf:type rdf:resource="http://www.w3.org/2002/07/owl#Class"/>
    <rdfs:subClassOf rdf:resource="http://www.openmath.org/ontology#Composite"/>
    <owl:disjointWith rdf:resource="http://www.openmath.org/ontology#ContentDictionaryGroup"/>
    <rdfs:isDefinedBy rdf:resource="http://www.openmath.org/ontology#"/>
  </rdf:Description>
  <rdf:Description rdf:nodeID="A13">
    <rdf:first rdf:resource="http://www.openmath.org/ontology#definesSymbol"/>
    <rdf:rest rdf:nodeID="A14"/>
  </rdf:Description>
  <rdf:Description rdf:nodeID="A4">
    <rdf:first rdf:resource="http://www.openmath.org/ontology#Application"/>
    <rdf:rest rdf:nodeID="A15"/>
  </rdf:Description>
  <rdf:Description rdf:about="http://www.openmath.org/ontology#url">
    <rdf:type rdf:resource="http://www.w3.org/2002/07/owl#ObjectProperty"/>
    <rdf:type rdf:resource="http://www.w3.org/2002/07/owl#FunctionalProperty"/>
    <rdfs:domain rdf:nodeID="A16"/>
    <rdfs:comment>The URL of a content dictionary or content dictionary group, as described in section 4.3.2 or 4.4.2.2, resp.</rdfs:comment>
    <rdfs:isDefinedBy rdf:resource="http://www.openmath.org/ontology#"/>
  </rdf:Description>
  <rdf:Description rdf:about="http://www.openmath.org/ontology#hasNotationDefinition">
    <rdf:type rdf:resource="http://www.w3.org/2002/07/owl#ObjectProperty"/>
    <rdf:type rdf:resource="http://www.w3.org/2002/07/owl#InverseFunctionalProperty"/>
    <owl:inverseOf rdf:resource="http://www.openmath.org/ontology#rendersSymbol"/>
    <rdfs:isDefinedBy rdf:resource="http://www.openmath.org/ontology#"/>
  </rdf:Description>
  <rdf:Description rdf:about="http://www.openmath.org/ontology#Binder">
    <rdf:type rdf:resource="http://www.openmath.org/ontology#Role"/>
    <rdfs:comment>The 'binder' role of a symbol, as described in section 2.1.4</rdfs:comment>
    <rdfs:isDefinedBy rdf:resource="http://www.openmath.org/ontology#"/>
  </rdf:Description>
  <rdf:Description rdf:nodeID="A7">
    <rdf:first rdf:resource="http://www.openmath.org/ontology#CommentedPart"/>
    <rdf:rest rdf:nodeID="A17"/>
  </rdf:Description>
  <rdf:Description rdf:about="http://www.openmath.org/ontology#Attribution">
    <rdf:type rdf:resource="http://www.openmath.org/ontology#Role"/>
    <rdfs:comment>The 'attribution' role of a symbol, as described in section 2.1.4</rdfs:comment>
    <rdfs:isDefinedBy rdf:resource="http://www.openmath.org/ontology#"/>
  </rdf:Description>
  <rdf:Description rdf:about="http://www.openmath.org/ontology#hasFormalPart">
    <rdf:type rdf:resource="http://www.w3.org/2002/07/owl#ObjectProperty"/>
    <rdf:type rdf:resource="http://www.w3.org/2002/07/owl#FunctionalProperty"/>
    <rdfs:subPropertyOf rdf:resource="http://www.openmath.org/ontology#hasDirectPart"/>
    <rdfs:domain rdf:resource="http://www.openmath.org/ontology#Property"/>
    <rdfs:range rdf:resource="http://www.openmath.org/ontology#FormalPart"/>
    <rdfs:comment>The relationship of a property container to its formal part (FMP).</rdfs:comment>
    <rdfs:isDefinedBy rdf:resource="http://www.openmath.org/ontology#"/>
  </rdf:Description>
  <rdf:Description rdf:about="http://purl.org/dc/terms/description">
    <rdf:type rdf:resource="http://www.w3.org/2002/07/owl#DatatypeProperty"/>
  </rdf:Description>
  <rdf:Description rdf:about="http://www.openmath.org/ontology#Version">
    <owl:disjointWith rdf:resource="http://www.openmath.org/ontology#Example"/>
    <owl:disjointWith rdf:resource="http://www.openmath.org/ontology#NotationDefinition"/>
    <rdfs:isDefinedBy rdf:resource="http://www.openmath.org/ontology#"/>
    <owl:disjointWith rdf:resource="http://www.openmath.org/ontology#CommentedPart"/>
    <owl:disjointWith rdf:resource="http://www.openmath.org/ontology#FormalPart"/>
    <owl:disjointWith rdf:resource="http://www.openmath.org/ontology#Status"/>
    <owl:disjointWith rdf:resource="http://www.openmath.org/ontology#Role"/>
    <rdfs:subClassOf rdf:nodeID="A18"/>
    <rdfs:subClassOf rdf:nodeID="A19"/>
    <rdfs:subClassOf rdf:nodeID="A20"/>
    <rdf:type rdf:resource="http://www.w3.org/2002/07/owl#Class"/>
    <rdfs:subClassOf rdf:nodeID="A21"/>
    <owl:disjointWith rdf:resource="http://www.openmath.org/ontology#Composite"/>
    <owl:disjointWith rdf:resource="http://www.openmath.org/ontology#CDBase"/>
    <rdfs:subClassOf rdf:resource="http://www.openmath.org/ontology#OpenMathConcept"/>
    <rdfs:comment>A version with major and minor part (both mandatory), as described in section 4.2, 4.3.2 or 4.4.2.2, resp.</rdfs:comment>
    <owl:disjointWith rdf:resource="http://www.openmath.org/ontology#Signature"/>
  </rdf:Description>
  <rdf:Description rdf:about="http://www.openmath.org/ontology#hasSignatureDictionary">
    <rdf:type rdf:resource="http://www.w3.org/2002/07/owl#ObjectProperty"/>
    <rdf:type rdf:resource="http://www.w3.org/2002/07/owl#InverseFunctionalProperty"/>
    <owl:inverseOf rdf:resource="http://www.openmath.org/ontology#containsSignaturesFor"/>
    <rdfs:isDefinedBy rdf:resource="http://www.openmath.org/ontology#"/>
  </rdf:Description>
  <rdf:Description rdf:about="http://www.openmath.org/ontology#FormalPart">
    <rdf:type rdf:resource="http://www.w3.org/2002/07/owl#Class"/>
    <rdfs:subClassOf rdf:resource="http://www.openmath.org/ontology#OpenMathConcept"/>
    <owl:disjointWith rdf:resource="http://www.openmath.org/ontology#Composite"/>
    <owl:disjointWith rdf:resource="http://www.openmath.org/ontology#CDBase"/>
    <owl:disjointWith rdf:resource="http://www.openmath.org/ontology#Status"/>
    <owl:disjointWith rdf:resource="http://www.openmath.org/ontology#Role"/>
    <owl:disjointWith rdf:resource="http://www.openmath.org/ontology#CommentedPart"/>
    <rdfs:comment>A formal part of a mathematical property (FMP) of a symbol, as described in sections 4.2 and 4.3</rdfs:comment>
    <rdfs:isDefinedBy rdf:resource="http://www.openmath.org/ontology#"/>
  </rdf:Description>
  <rdf:Description rdf:nodeID="A10">
    <rdf:type rdf:resource="http://www.w3.org/2002/07/owl#Restriction"/>
    <owl:onProperty rdf:resource="http://purl.org/dc/terms/identifier"/>
    <owl:allValuesFrom rdf:resource="http://www.w3.org/2001/XMLSchema#NCName"/>
  </rdf:Description>
  <rdf:Description rdf:about="http://www.openmath.org/ontology#exemplifies">
    <rdf:type rdf:resource="http://www.w3.org/2002/07/owl#ObjectProperty"/>
    <rdf:type rdf:resource="http://www.w3.org/2002/07/owl#FunctionalProperty"/>
    <owl:inverseOf rdf:resource="http://www.openmath.org/ontology#exemplifiedBy"/>
    <rdfs:isDefinedBy rdf:resource="http://www.openmath.org/ontology#"/>
  </rdf:Description>
  <rdf:Description rdf:about="http://www.openmath.org/ontology#hasPragmaticSyntax">
    <rdf:type rdf:resource="http://www.w3.org/2002/07/owl#ObjectProperty"/>
    <rdfs:subPropertyOf rdf:resource="http://www.openmath.org/ontology#hasDirectPart"/>
    <rdfs:comment>OpenMath 3 transitional</rdfs:comment>
    <rdfs:domain rdf:resource="http://www.openmath.org/ontology#SymbolDefinition"/>
    <rdfs:range rdf:resource="http://www.openmath.org/ontology#PragmaticSyntax"/>
    <rdfs:comment>The relationship of a symbol definition to its pragmatic usage guidelines</rdfs:comment>
    <rdfs:isDefinedBy rdf:resource="http://www.openmath.org/ontology#"/>
  </rdf:Description>
  <rdf:Description rdf:about="http://www.openmath.org/ontology#usesDirectly">
    <rdf:type rdf:resource="http://www.w3.org/2002/07/owl#ObjectProperty"/>
    <rdfs:subPropertyOf rdf:resource="http://www.openmath.org/ontology#uses"/>
    <rdfs:domain rdf:resource="http://www.openmath.org/ontology#ContentDictionary"/>
    <rdfs:range rdf:resource="http://www.openmath.org/ontology#ContentDictionary"/>
    <owl:propertyChainAxiom rdf:nodeID="A22"/>
    <owl:propertyChainAxiom rdf:nodeID="A13"/>
    <rdfs:comment>Other content dictionaries directly used by this one, as described in section 4.3.2</rdfs:comment>
    <rdfs:isDefinedBy rdf:resource="http://www.openmath.org/ontology#"/>
  </rdf:Description>
  <rdf:Description rdf:about="http://www.openmath.org/ontology#Property">
    <rdf:type rdf:resource="http://www.w3.org/2002/07/owl#Class"/>
    <rdfs:subClassOf rdf:resource="http://www.openmath.org/ontology#Composite"/>
    <owl:disjointWith rdf:resource="http://www.openmath.org/ontology#ContentDictionaryGroup"/>
    <owl:disjointWith rdf:resource="http://www.openmath.org/ontology#Dictionary"/>
    <owl:disjointWith rdf:resource="http://www.openmath.org/ontology#SymbolDefinition"/>
    <rdfs:comment>A mathematical property of a symbol, can have a commented (CMP), a formal (FMP) part, or both; cf. sections 4.2 and 4.3</rdfs:comment>
    <rdfs:isDefinedBy rdf:resource="http://www.openmath.org/ontology#"/>
  </rdf:Description>
  <rdf:Description rdf:nodeID="A14">
    <rdf:first rdf:resource="http://www.openmath.org/ontology#exemplifiedBy"/>
    <rdf:rest rdf:nodeID="A23"/>
  </rdf:Description>
  <rdf:Description rdf:nodeID="A24">
    <rdf:first rdf:resource="http://www.openmath.org/ontology#Attribution"/>
    <rdf:rest rdf:nodeID="A25"/>
  </rdf:Description>
  <rdf:Description rdf:nodeID="A26">
    <rdf:first rdf:resource="http://www.openmath.org/ontology#ContentDictionary"/>
    <rdf:rest rdf:nodeID="A27"/>
  </rdf:Description>
  <rdf:Description rdf:about="http://www.openmath.org/ontology#containsContentDictionary">
    <rdf:type rdf:resource="http://www.w3.org/2002/07/owl#ObjectProperty"/>
    <rdfs:subPropertyOf rdf:resource="http://www.openmath.org/ontology#comprises"/>
    <rdfs:domain rdf:resource="http://www.openmath.org/ontology#ContentDictionaryGroup"/>
    <rdfs:range rdf:resource="http://www.openmath.org/ontology#ContentDictionary"/>
    <rdfs:comment>The relationship of a content dictionary group to a content dictionary it contains</rdfs:comment>
    <rdfs:isDefinedBy rdf:resource="http://www.openmath.org/ontology#"/>
  </rdf:Description>
  <rdf:Description rdf:nodeID="A28">
    <rdf:first rdf:resource="http://www.openmath.org/ontology#usesSymbol"/>
    <rdf:rest rdf:nodeID="A29"/>
  </rdf:Description>
  <rdf:Description rdf:about="http://www.openmath.org/ontology#definesSymbol">
    <rdf:type rdf:resource="http://www.w3.org/2002/07/owl#ObjectProperty"/>
    <rdfs:subPropertyOf rdf:resource="http://www.openmath.org/ontology#hasDirectPart"/>
    <rdfs:domain rdf:resource="http://www.openmath.org/ontology#ContentDictionary"/>
    <rdfs:range rdf:resource="http://www.openmath.org/ontology#SymbolDefinition"/>
    <owl:inverseOf rdf:resource="http://www.openmath.org/ontology#definedIn"/>
    <rdfs:comment>The relationship of a content dictionary to a symbol it defines</rdfs:comment>
    <rdfs:isDefinedBy rdf:resource="http://www.openmath.org/ontology#"/>
  </rdf:Description>
  <rdf:Description rdf:about="http://purl.org/dc/terms/subject">
    <rdf:type rdf:resource="http://www.w3.org/2002/07/owl#AnnotationProperty"/>
  </rdf:Description>
  <rdf:Description rdf:about="http://www.openmath.org/ontology#uses">
    <rdf:type rdf:resource="http://www.w3.org/2002/07/owl#ObjectProperty"/>
    <rdf:type rdf:resource="http://www.w3.org/2002/07/owl#TransitiveProperty"/>
    <rdfs:subPropertyOf rdf:resource="http://omdoc.org/ontology#dependsOn"/>
    <rdfs:isDefinedBy rdf:resource="http://www.openmath.org/ontology#"/>
  </rdf:Description>
  <rdf:Description rdf:about="http://www.openmath.org/ontology#status">
    <rdf:type rdf:resource="http://www.w3.org/2002/07/owl#ObjectProperty"/>
    <rdf:type rdf:resource="http://www.w3.org/2002/07/owl#FunctionalProperty"/>
    <rdfs:domain rdf:resource="http://www.openmath.org/ontology#Dictionary"/>
    <rdfs:range rdf:resource="http://www.openmath.org/ontology#Status"/>
    <rdfs:comment>The status of a content dictionary or signature dictionary, as described in section 4.2.1 and 4.3.2</rdfs:comment>
    <rdfs:isDefinedBy rdf:resource="http://www.openmath.org/ontology#"/>
  </rdf:Description>
  <rdf:Description rdf:about="http://www.openmath.org/ontology#minor">
    <rdf:type rdf:resource="http://www.w3.org/2002/07/owl#DatatypeProperty"/>
    <rdf:type rdf:resource="http://www.w3.org/2002/07/owl#FunctionalProperty"/>
    <rdfs:domain rdf:resource="http://www.openmath.org/ontology#Version"/>
    <rdfs:range rdf:resource="http://www.w3.org/2001/XMLSchema#nonNegativeInteger"/>
    <rdfs:comment>Minor part of a version number, as described in section 4.2.2</rdfs:comment>
    <rdfs:isDefinedBy rdf:resource="http://www.openmath.org/ontology#"/>
  </rdf:Description>
  <rdf:Description rdf:nodeID="A9">
    <rdf:type rdf:resource="http://www.w3.org/2002/07/owl#Restriction"/>
    <owl:onProperty rdf:resource="http://purl.org/dc/terms/description"/>
    <owl:cardinality rdf:datatype="http://www.w3.org/2001/XMLSchema#nonNegativeInteger">1</owl:cardinality>
  </rdf:Description>
  <rdf:Description rdf:nodeID="A23">
    <rdf:first rdf:resource="http://www.openmath.org/ontology#usesSymbol"/>
    <rdf:rest rdf:nodeID="A30"/>
  </rdf:Description>
  <rdf:Description rdf:about="http://www.openmath.org/ontology#Example">
    <owl:disjointWith rdf:resource="http://www.openmath.org/ontology#Composite"/>
    <rdfs:subClassOf rdf:resource="http://www.openmath.org/ontology#OpenMathConcept"/>
    <owl:disjointWith rdf:resource="http://www.openmath.org/ontology#Role"/>
    <rdf:type rdf:resource="http://www.w3.org/2002/07/owl#Class"/>
    <rdfs:comment>An example for a symbol, as described in sections 4.2 and 4.3</rdfs:comment>
    <owl:disjointWith rdf:resource="http://www.openmath.org/ontology#Status"/>
    <rdfs:isDefinedBy rdf:resource="http://www.openmath.org/ontology#"/>
    <owl:disjointWith rdf:resource="http://www.openmath.org/ontology#CDBase"/>
    <owl:disjointWith rdf:resource="http://www.openmath.org/ontology#FormalPart"/>
    <owl:disjointWith rdf:resource="http://www.openmath.org/ontology#CommentedPart"/>
  </rdf:Description>
  <rdf:Description rdf:nodeID="A25">
    <rdf:first rdf:resource="http://www.openmath.org/ontology#SemanticAttribution"/>
    <rdf:rest rdf:nodeID="A3"/>
  </rdf:Description>
  <rdf:Description rdf:nodeID="A29">
    <rdf:first rdf:resource="http://www.openmath.org/ontology#definedIn"/>
    <rdf:rest rdf:resource="http://www.w3.org/1999/02/22-rdf-syntax-ns#nil"/>
  </rdf:Description>
  <rdf:Description rdf:about="http://www.openmath.org/ontology#Constant">
    <rdf:type rdf:resource="http://www.openmath.org/ontology#Role"/>
    <rdfs:comment>The 'constant' role of a symbol, as described in section 2.1.4</rdfs:comment>
    <rdfs:isDefinedBy rdf:resource="http://www.openmath.org/ontology#"/>
  </rdf:Description>
  <rdf:Description rdf:about="http://www.openmath.org/ontology#SignatureDictionary">
    <rdf:type rdf:resource="http://www.w3.org/2002/07/owl#Class"/>
    <rdfs:subClassOf rdf:resource="http://www.openmath.org/ontology#Dictionary"/>
    <owl:disjointWith rdf:resource="http://www.openmath.org/ontology#ContentDictionary"/>
    <rdfs:comment>An OpenMath Signature Dictionary, as described in section 4.4.  Some of the properties of signature dictionaries are defined as properties in this ontology, others are taken from Dublin Core and RDFS, with the following mapping: Name = dct:identifier</rdfs:comment>
    <rdfs:isDefinedBy rdf:resource="http://www.openmath.org/ontology#"/>
  </rdf:Description>
  <rdf:Description rdf:about="http://www.openmath.org/ontology#Signature">
    <rdf:type rdf:resource="http://www.w3.org/2002/07/owl#Class"/>
    <owl:disjointWith rdf:resource="http://www.openmath.org/ontology#FormalPart"/>
    <rdfs:comment>A type signature of a symbol, as described in section 4.4</rdfs:comment>
    <owl:disjointWith rdf:resource="http://www.openmath.org/ontology#CommentedPart"/>
    <owl:disjointWith rdf:resource="http://www.openmath.org/ontology#Example"/>
    <owl:disjointWith rdf:resource="http://www.openmath.org/ontology#Status"/>
    <rdfs:isDefinedBy rdf:resource="http://www.openmath.org/ontology#"/>
    <owl:disjointWith rdf:resource="http://www.openmath.org/ontology#Composite"/>
    <rdfs:subClassOf rdf:resource="http://www.openmath.org/ontology#OpenMathConcept"/>
    <owl:disjointWith rdf:resource="http://www.openmath.org/ontology#CDBase"/>
    <owl:disjointWith rdf:resource="http://www.openmath.org/ontology#Role"/>
  </rdf:Description>
  <rdf:Description rdf:nodeID="A27">
    <rdf:first rdf:resource="http://www.openmath.org/ontology#ContentDictionaryGroup"/>
    <rdf:rest rdf:resource="http://www.w3.org/1999/02/22-rdf-syntax-ns#nil"/>
  </rdf:Description>
  <rdf:Description rdf:about="http://www.openmath.org/ontology#base">
    <rdf:type rdf:resource="http://www.w3.org/2002/07/owl#ObjectProperty"/>
    <rdf:type rdf:resource="http://www.w3.org/2002/07/owl#FunctionalProperty"/>
    <rdfs:domain rdf:resource="http://www.openmath.org/ontology#ContentDictionary"/>
    <rdfs:range rdf:resource="http://www.openmath.org/ontology#CDBase"/>
    <rdfs:comment>The CD base URI of a content dictionary, as described in section 4.3.2</rdfs:comment>
    <rdfs:isDefinedBy rdf:resource="http://www.openmath.org/ontology#"/>
  </rdf:Description>
  <rdf:Description rdf:nodeID="A31">
    <rdf:type rdf:resource="http://www.w3.org/2002/07/owl#Restriction"/>
    <owl:onProperty rdf:resource="http://www.openmath.org/ontology#reviewDate"/>
    <owl:cardinality rdf:datatype="http://www.w3.org/2001/XMLSchema#nonNegativeInteger">1</owl:cardinality>
  </rdf:Description>
  <rdf:Description rdf:nodeID="A32">
    <rdf:type rdf:resource="http://www.w3.org/2002/07/owl#Restriction"/>
    <owl:onProperty rdf:resource="http://www.openmath.org/ontology#definesSymbol"/>
    <owl:minCardinality rdf:datatype="http://www.w3.org/2001/XMLSchema#nonNegativeInteger">1</owl:minCardinality>
  </rdf:Description>
  <rdf:Description rdf:about="http://www.openmath.org/ontology#hasProperty">
    <rdf:type rdf:resource="http://www.w3.org/2002/07/owl#ObjectProperty"/>
    <rdfs:subPropertyOf rdf:resource="http://www.openmath.org/ontology#hasDirectPart"/>
    <rdfs:domain rdf:resource="http://www.openmath.org/ontology#SymbolDefinition"/>
    <rdfs:range rdf:resource="http://www.openmath.org/ontology#Property"/>
    <rdfs:comment>The relationship of a symbol definition to a CMP or FMP (OpenMath 2) or a property container that it contains</rdfs:comment>
    <rdfs:isDefinedBy rdf:resource="http://www.openmath.org/ontology#"/>
  </rdf:Description>
  <rdf:Description rdf:nodeID="A30">
    <rdf:first rdf:resource="http://www.openmath.org/ontology#definedIn"/>
    <rdf:rest rdf:resource="http://www.w3.org/1999/02/22-rdf-syntax-ns#nil"/>
  </rdf:Description>
  <rdf:Description rdf:about="http://www.openmath.org/ontology#role">
    <rdf:type rdf:resource="http://www.w3.org/2002/07/owl#ObjectProperty"/>
    <rdf:type rdf:resource="http://www.w3.org/2002/07/owl#FunctionalProperty"/>
    <rdfs:domain rdf:resource="http://www.openmath.org/ontology#SymbolDefinition"/>
    <rdfs:range rdf:resource="http://www.openmath.org/ontology#Role"/>
    <rdfs:comment>The role of a symbol, as described in section 4.3.2</rdfs:comment>
    <rdfs:isDefinedBy rdf:resource="http://www.openmath.org/ontology#"/>
  </rdf:Description>
  <rdf:Description rdf:about="http://www.openmath.org/ontology#NotationDictionary">
    <rdf:type rdf:resource="http://www.w3.org/2002/07/owl#Class"/>
    <rdfs:subClassOf rdf:resource="http://www.openmath.org/ontology#Dictionary"/>
    <owl:disjointWith rdf:resource="http://www.openmath.org/ontology#ContentDictionary"/>
    <owl:disjointWith rdf:resource="http://www.openmath.org/ontology#SignatureDictionary"/>
    <rdfs:comment>This is not (yet) an official part of the OpenMath standard.  This name was conceived in analogy to “Content Dictionaries” and “Signature Dictionaries”.</rdfs:comment>
    <rdfs:isDefinedBy rdf:resource="http://www.openmath.org/ontology#"/>
  </rdf:Description>
  <rdf:Description rdf:nodeID="A33">
    <rdf:type rdf:resource="http://www.w3.org/2002/07/owl#Restriction"/>
    <owl:onProperty rdf:resource="http://purl.org/dc/terms/date"/>
    <owl:allValuesFrom rdf:resource="http://www.w3.org/2001/XMLSchema#date"/>
  </rdf:Description>
  <rdf:Description rdf:about="http://www.openmath.org/ontology#CDBase">
    <rdf:type rdf:resource="http://www.w3.org/2002/07/owl#Class"/>
    <rdfs:subClassOf rdf:resource="http://www.openmath.org/ontology#OpenMathConcept"/>
    <owl:disjointWith rdf:resource="http://www.openmath.org/ontology#Composite"/>
    <rdfs:comment>An OpenMath Content Dictionary base URI, as described in sections 2.3 and 4.2</rdfs:comment>
    <rdfs:isDefinedBy rdf:resource="http://www.openmath.org/ontology#"/>
  </rdf:Description>
  <rdf:Description rdf:about="http://www.openmath.org/ontology#Role">
    <rdf:type rdf:resource="http://www.w3.org/2002/07/owl#Class"/>
    <rdfs:subClassOf rdf:resource="http://www.openmath.org/ontology#OpenMathConcept"/>
    <owl:disjointWith rdf:resource="http://www.openmath.org/ontology#Composite"/>
    <owl:disjointWith rdf:resource="http://www.openmath.org/ontology#CDBase"/>
    <owl:disjointWith rdf:resource="http://www.openmath.org/ontology#Status"/>
    <rdfs:comment>The role of a symbol, as described in sections 2.1.4 and 4.3.2</rdfs:comment>
    <owl:oneOf rdf:nodeID="A34"/>
    <rdfs:isDefinedBy rdf:resource="http://www.openmath.org/ontology#"/>
  </rdf:Description>
  <rdf:Description rdf:nodeID="A16">
    <owl:unionOf rdf:nodeID="A35"/>
  </rdf:Description>
  <rdf:Description rdf:nodeID="A18">
    <rdf:type rdf:resource="http://www.w3.org/2002/07/owl#Restriction"/>
    <owl:onProperty rdf:resource="http://www.openmath.org/ontology#major"/>
    <owl:cardinality rdf:datatype="http://www.w3.org/2001/XMLSchema#nonNegativeInteger">1</owl:cardinality>
  </rdf:Description>
  <rdf:Description rdf:about="http://www.openmath.org/ontology#Error">
    <rdf:type rdf:resource="http://www.openmath.org/ontology#Role"/>
    <rdfs:comment>The 'error' role of a symbol, as described in section 2.1.4</rdfs:comment>
    <rdfs:isDefinedBy rdf:resource="http://www.openmath.org/ontology#"/>
  </rdf:Description>
  <rdf:Description rdf:about="http://www.openmath.org/ontology#containsSignaturesFor">
    <rdf:type rdf:resource="http://www.w3.org/2002/07/owl#ObjectProperty"/>
    <rdf:type rdf:resource="http://www.w3.org/2002/07/owl#FunctionalProperty"/>
    <rdfs:domain rdf:resource="http://www.openmath.org/ontology#SignatureDictionary"/>
    <rdfs:range rdf:resource="http://www.openmath.org/ontology#ContentDictionary"/>
    <rdfs:comment>The relationship of a signature dictionary to the content dictionary whose symbols it specifies</rdfs:comment>
    <rdfs:isDefinedBy rdf:resource="http://www.openmath.org/ontology#"/>
  </rdf:Description>
  <rdf:Description rdf:nodeID="A11">
    <rdf:type rdf:resource="http://www.w3.org/2002/07/owl#Restriction"/>
    <owl:onProperty rdf:resource="http://purl.org/dc/terms/identifier"/>
    <owl:cardinality rdf:datatype="http://www.w3.org/2001/XMLSchema#nonNegativeInteger">1</owl:cardinality>
  </rdf:Description>
  <rdf:Description rdf:about="http://www.openmath.org/ontology#definedIn">
    <rdf:type rdf:resource="http://www.w3.org/2002/07/owl#ObjectProperty"/>
    <owl:inverseOf rdf:resource="http://www.openmath.org/ontology#definesSymbol"/>
    <rdfs:comment>The relationship of a symbol definition to its enclosing content dictionary</rdfs:comment>
    <rdfs:isDefinedBy rdf:resource="http://www.openmath.org/ontology#"/>
  </rdf:Description>
  <rdf:Description rdf:nodeID="A36">
    <rdf:type rdf:resource="http://www.w3.org/2002/07/owl#Restriction"/>
    <owl:onProperty rdf:resource="http://www.openmath.org/ontology#reviewDate"/>
    <owl:allValuesFrom rdf:resource="http://www.w3.org/2001/XMLSchema#date"/>
  </rdf:Description>
  <rdf:Description rdf:nodeID="A37">
    <rdf:type rdf:resource="http://www.w3.org/2002/07/owl#Restriction"/>
    <owl:onProperty rdf:resource="http://purl.org/dc/terms/date"/>
    <owl:cardinality rdf:datatype="http://www.w3.org/2001/XMLSchema#nonNegativeInteger">1</owl:cardinality>
  </rdf:Description>
  <rdf:Description rdf:nodeID="A22">
    <rdf:first rdf:resource="http://www.openmath.org/ontology#definesSymbol"/>
    <rdf:rest rdf:nodeID="A38"/>
  </rdf:Description>
  <rdf:Description rdf:about="http://www.openmath.org/ontology#Application">
    <rdf:type rdf:resource="http://www.openmath.org/ontology#Role"/>
    <rdfs:comment>The 'application' role of a symbol, as described in section 2.1.4</rdfs:comment>
    <rdfs:isDefinedBy rdf:resource="http://www.openmath.org/ontology#"/>
  </rdf:Description>
  <rdf:Description rdf:nodeID="A39">
    <owl:unionOf rdf:nodeID="A26"/>
  </rdf:Description>
  <rdf:Description rdf:nodeID="A35">
    <rdf:first rdf:resource="http://www.openmath.org/ontology#ContentDictionary"/>
    <rdf:rest rdf:nodeID="A40"/>
  </rdf:Description>
  <rdf:Description rdf:about="http://www.openmath.org/ontology#ContentDictionaryGroup">
    <rdf:type rdf:resource="http://www.w3.org/2002/07/owl#Class"/>
    <rdfs:subClassOf rdf:resource="http://www.openmath.org/ontology#Composite"/>
    <rdfs:comment>An OpenMath CD (Content Dictionary) Group, as described in section 4.4.2.  Some of the properties of content dictionaries are defined as properties in this ontology, others are taken from Dublin Core and RDFS, with the following mapping: CDGroupName = dct:identifier, CDGroupDescription = dct:description, CDComment = rdfs:comment.</rdfs:comment>
    <rdfs:isDefinedBy rdf:resource="http://www.openmath.org/ontology#"/>
  </rdf:Description>
  <rdf:Description rdf:nodeID="A41">
    <rdf:type rdf:resource="http://www.w3.org/2002/07/owl#Restriction"/>
    <owl:onProperty rdf:resource="http://www.openmath.org/ontology#version"/>
    <owl:cardinality rdf:datatype="http://www.w3.org/2001/XMLSchema#nonNegativeInteger">1</owl:cardinality>
  </rdf:Description>
  <rdf:Description rdf:about="http://www.openmath.org/ontology#containsNotationDefinition">
    <rdf:type rdf:resource="http://www.w3.org/2002/07/owl#ObjectProperty"/>
    <rdfs:subPropertyOf rdf:resource="http://www.openmath.org/ontology#hasDirectPart"/>
    <rdfs:domain rdf:resource="http://www.openmath.org/ontology#NotationDictionary"/>
    <rdfs:range rdf:resource="http://www.openmath.org/ontology#NotationDefinition"/>
    <rdfs:comment>The relationship of a notation dictionary to a notation definition it contains</rdfs:comment>
    <rdfs:isDefinedBy rdf:resource="http://www.openmath.org/ontology#"/>
  </rdf:Description>
  <rdf:Description rdf:about="http://www.openmath.org/ontology#containsSignature">
    <rdf:type rdf:resource="http://www.w3.org/2002/07/owl#ObjectProperty"/>
    <rdfs:subPropertyOf rdf:resource="http://www.openmath.org/ontology#hasDirectPart"/>
    <rdfs:domain rdf:resource="http://www.openmath.org/ontology#SignatureDictionary"/>
    <rdfs:range rdf:resource="http://www.openmath.org/ontology#Signature"/>
    <rdfs:comment>The relationship of a signature dictionary to a type signature it contains</rdfs:comment>
    <rdfs:isDefinedBy rdf:resource="http://www.openmath.org/ontology#"/>
  </rdf:Description>
  <rdf:Description rdf:nodeID="A17">
    <rdf:first rdf:resource="http://www.openmath.org/ontology#Example"/>
    <rdf:rest rdf:resource="http://www.w3.org/1999/02/22-rdf-syntax-ns#nil"/>
  </rdf:Description>
  <rdf:Description rdf:nodeID="A42">
    <rdf:type rdf:resource="http://www.w3.org/2002/07/owl#Restriction"/>
    <owl:onProperty rdf:resource="http://purl.org/dc/terms/description"/>
    <owl:cardinality rdf:datatype="http://www.w3.org/2001/XMLSchema#nonNegativeInteger">1</owl:cardinality>
  </rdf:Description>
  <rdf:Description rdf:about="http://www.openmath.org/ontology#containsNotationsFor">
    <rdf:type rdf:resource="http://www.w3.org/2002/07/owl#ObjectProperty"/>
    <rdf:type rdf:resource="http://www.w3.org/2002/07/owl#FunctionalProperty"/>
    <rdfs:domain rdf:resource="http://www.openmath.org/ontology#NotationDictionary"/>
    <rdfs:range rdf:resource="http://www.openmath.org/ontology#ContentDictionary"/>
    <rdfs:comment>The relationship of a notation dictionary to the content dictionary whose symbols it specifies</rdfs:comment>
    <rdfs:isDefinedBy rdf:resource="http://www.openmath.org/ontology#"/>
  </rdf:Description>
  <rdf:Description rdf:about="http://www.openmath.org/ontology#major">
    <rdf:type rdf:resource="http://www.w3.org/2002/07/owl#DatatypeProperty"/>
    <rdf:type rdf:resource="http://www.w3.org/2002/07/owl#FunctionalProperty"/>
    <rdfs:domain rdf:resource="http://www.openmath.org/ontology#Version"/>
    <rdfs:range rdf:resource="http://www.w3.org/2001/XMLSchema#nonNegativeInteger"/>
    <rdfs:comment>Major part of a version number, as described in section 4.2.2</rdfs:comment>
    <rdfs:isDefinedBy rdf:resource="http://www.openmath.org/ontology#"/>
  </rdf:Description>
  <rdf:Description rdf:about="http://www.openmath.org/ontology#Composite">
    <rdf:type rdf:resource="http://www.w3.org/2002/07/owl#Class"/>
    <rdfs:subClassOf rdf:resource="http://www.openmath.org/ontology#OpenMathConcept"/>
    <rdfs:comment>The generic superclass of all concepts that can be expressed in OpenMath content/signature/notation dictionaries and that can comprise subconcepts</rdfs:comment>
    <rdfs:isDefinedBy rdf:resource="http://www.openmath.org/ontology#"/>
  </rdf:Description>
  <rdf:Description rdf:about="http://purl.org/dc/terms/date">
    <rdf:type rdf:resource="http://www.w3.org/2002/07/owl#DatatypeProperty"/>
  </rdf:Description>
  <rdf:Description rdf:nodeID="A38">
    <rdf:first rdf:resource="http://www.openmath.org/ontology#hasProperty"/>
    <rdf:rest rdf:nodeID="A43"/>
  </rdf:Description>
  <rdf:Description rdf:about="http://www.openmath.org/ontology#exemplifiedBy">
    <rdf:type rdf:resource="http://www.w3.org/2002/07/owl#ObjectProperty"/>
    <rdfs:subPropertyOf rdf:resource="http://www.openmath.org/ontology#hasDirectPart"/>
    <rdfs:domain rdf:resource="http://www.openmath.org/ontology#SymbolDefinition"/>
    <rdfs:range rdf:resource="http://www.openmath.org/ontology#Example"/>
    <rdfs:comment>The relationship of a symbol definition to an example it contains</rdfs:comment>
    <rdfs:isDefinedBy rdf:resource="http://www.openmath.org/ontology#"/>
  </rdf:Description>
  <rdf:Description rdf:about="http://www.openmath.org/ontology#rendersSymbol">
    <rdf:type rdf:resource="http://www.w3.org/2002/07/owl#ObjectProperty"/>
    <rdf:type rdf:resource="http://www.w3.org/2002/07/owl#FunctionalProperty"/>
    <rdfs:domain rdf:resource="http://www.openmath.org/ontology#NotationDefinition"/>
    <rdfs:range rdf:resource="http://www.openmath.org/ontology#SymbolDefinition"/>
    <rdfs:comment>The relationship of a notation definition to the symbol it renders</rdfs:comment>
    <rdfs:isDefinedBy rdf:resource="http://www.openmath.org/ontology#"/>
  </rdf:Description>
  <rdf:Description rdf:nodeID="A44">
    <rdf:first rdf:resource="http://www.openmath.org/ontology#ContentDictionaryGroup"/>
    <rdf:rest rdf:resource="http://www.w3.org/1999/02/22-rdf-syntax-ns#nil"/>
  </rdf:Description>
  <rdf:Description rdf:nodeID="A12">
    <owl:unionOf rdf:nodeID="A45"/>
  </rdf:Description>
  <rdf:Description rdf:about="http://www.openmath.org/ontology#version">
    <rdf:type rdf:resource="http://www.w3.org/2002/07/owl#DatatypeProperty"/>
    <rdf:type rdf:resource="http://www.w3.org/2002/07/owl#FunctionalProperty"/>
    <rdfs:domain rdf:nodeID="A39"/>
    <rdfs:range rdf:resource="http://www.openmath.org/ontology#Version"/>
    <rdfs:comment>The version of a content dictionary or content dictionary group, as described in sections 4.2.2 and 4.3.2 or 4.4.2.2, resp.</rdfs:comment>
    <rdfs:isDefinedBy rdf:resource="http://www.openmath.org/ontology#"/>
  </rdf:Description>
  <rdf:Description rdf:about="http://purl.org/dc/terms/title">
    <rdf:type rdf:resource="http://www.w3.org/2002/07/owl#AnnotationProperty"/>
  </rdf:Description>
  <rdf:Description rdf:nodeID="A40">
    <rdf:first rdf:resource="http://www.openmath.org/ontology#ContentDictionaryGroup"/>
    <rdf:rest rdf:resource="http://www.w3.org/1999/02/22-rdf-syntax-ns#nil"/>
  </rdf:Description>
  <rdf:Description rdf:about="http://www.openmath.org/ontology#typesSymbol">
    <rdf:type rdf:resource="http://www.w3.org/2002/07/owl#ObjectProperty"/>
    <rdf:type rdf:resource="http://www.w3.org/2002/07/owl#FunctionalProperty"/>
    <rdfs:domain rdf:resource="http://www.openmath.org/ontology#Signature"/>
    <rdfs:range rdf:resource="http://www.openmath.org/ontology#SymbolDefinition"/>
    <rdfs:comment>The relationship of a type signature to the symbol it specifies</rdfs:comment>
    <rdfs:isDefinedBy rdf:resource="http://www.openmath.org/ontology#"/>
  </rdf:Description>
  <rdf:Description rdf:nodeID="A46">
    <rdf:first rdf:resource="http://www.openmath.org/ontology#Experimental"/>
    <rdf:rest rdf:nodeID="A47"/>
  </rdf:Description>
  <rdf:Description rdf:nodeID="A15">
    <rdf:first rdf:resource="http://www.openmath.org/ontology#Constant"/>
    <rdf:rest rdf:resource="http://www.w3.org/1999/02/22-rdf-syntax-ns#nil"/>
  </rdf:Description>
  <rdf:Description rdf:nodeID="A20">
    <rdf:type rdf:resource="http://www.w3.org/2002/07/owl#Restriction"/>
    <owl:onProperty rdf:resource="http://www.openmath.org/ontology#minor"/>
    <owl:cardinality rdf:datatype="http://www.w3.org/2001/XMLSchema#nonNegativeInteger">1</owl:cardinality>
  </rdf:Description>
  <rdf:Description rdf:about="http://www.openmath.org/ontology#hasPart">
    <rdf:type rdf:resource="http://www.w3.org/2002/07/owl#TransitiveProperty"/>
    <rdf:type rdf:resource="http://www.w3.org/2002/07/owl#ObjectProperty"/>
    <rdfs:subPropertyOf rdf:resource="http://www.openmath.org/ontology#comprises"/>
    <rdfs:subPropertyOf rdf:resource="http://omdoc.org/ontology#hasPart"/>
    <rdfs:comment>This relation denotes that one concept A, directly or indirectly, logically contains another concept B, and that B is not contained by any other concept than A, as reflected by child elements in OpenMath XML documents.</rdfs:comment>
    <rdfs:isDefinedBy rdf:resource="http://www.openmath.org/ontology#"/>
  </rdf:Description>
  <rdf:Description rdf:about="http://purl.org/dc/terms/contributor">
    <rdf:type rdf:resource="http://www.w3.org/2002/07/owl#AnnotationProperty"/>
  </rdf:Description>
  <rdf:Description rdf:nodeID="A48">
    <rdf:type rdf:resource="http://www.w3.org/2002/07/owl#Restriction"/>
    <owl:onProperty rdf:resource="http://www.openmath.org/ontology#status"/>
    <owl:cardinality rdf:datatype="http://www.w3.org/2001/XMLSchema#nonNegativeInteger">1</owl:cardinality>
  </rdf:Description>
  <rdf:Description rdf:nodeID="A34">
    <rdf:first rdf:resource="http://www.openmath.org/ontology#Binder"/>
    <rdf:rest rdf:nodeID="A24"/>
  </rdf:Description>
  <rdf:Description rdf:about="http://www.openmath.org/ontology#PragmaticSyntax">
    <rdf:type rdf:resource="http://www.w3.org/2002/07/owl#Class"/>
    <rdfs:subClassOf rdf:resource="http://www.openmath.org/ontology#Composite"/>
    <owl:disjointWith rdf:resource="http://www.openmath.org/ontology#ContentDictionaryGroup"/>
    <owl:disjointWith rdf:resource="http://www.openmath.org/ontology#Dictionary"/>
    <owl:disjointWith rdf:resource="http://www.openmath.org/ontology#SymbolDefinition"/>
    <owl:disjointWith rdf:resource="http://www.openmath.org/ontology#Property"/>
    <rdfs:comment>OpenMath 3 transitional</rdfs:comment>
    <rdfs:comment>Guidelines for using this symbol in pragmatic Content MathML</rdfs:comment>
    <rdfs:isDefinedBy rdf:resource="http://www.openmath.org/ontology#"/>
  </rdf:Description>
  <rdf:Description rdf:about="http://www.openmath.org/ontology#ContentDictionary">
    <rdfs:subClassOf rdf:nodeID="A36"/>
    <rdfs:subClassOf rdf:nodeID="A33"/>
    <rdfs:comment>OpenMath 3 transitional aspects: Title = dct:title</rdfs:comment>
    <rdfs:subClassOf rdf:nodeID="A31"/>
    <rdf:type rdf:resource="http://www.w3.org/2002/07/owl#Class"/>
    <rdfs:subClassOf rdf:nodeID="A48"/>
    <rdfs:subClassOf rdf:nodeID="A49"/>
    <rdfs:subClassOf rdf:nodeID="A42"/>
    <rdfs:subClassOf rdf:nodeID="A37"/>
    <rdfs:subClassOf rdf:nodeID="A32"/>
    <rdfs:subClassOf rdf:resource="http://www.openmath.org/ontology#Dictionary"/>
    <rdfs:isDefinedBy rdf:resource="http://www.openmath.org/ontology#"/>
    <rdfs:subClassOf rdf:nodeID="A50"/>
    <rdfs:subClassOf rdf:nodeID="A41"/>
    <rdfs:comment>An OpenMath Content Dictionary, as described in chapter 4.  Some of the properties of content dictionaries are defined as properties in this ontology, others are taken from Dublin Core and RDFS, with the following mapping: CDName = dct:identifier, Title = dct:title, Description = dct:description, CDDate = dct:date, CDComment = rdfs:comment.</rdfs:comment>
  </rdf:Description>
  <rdf:Description rdf:nodeID="A50">
    <rdf:type rdf:resource="http://www.w3.org/2002/07/owl#Restriction"/>
    <owl:onProperty rdf:resource="http://purl.org/dc/terms/identifier"/>
    <owl:allValuesFrom rdf:resource="http://www.w3.org/2001/XMLSchema#NCName"/>
  </rdf:Description>
  <rdf:Description rdf:about="http://www.openmath.org/ontology#Status">
    <rdf:type rdf:resource="http://www.w3.org/2002/07/owl#Class"/>
    <rdfs:subClassOf rdf:resource="http://www.openmath.org/ontology#OpenMathConcept"/>
    <owl:disjointWith rdf:resource="http://www.openmath.org/ontology#Composite"/>
    <owl:disjointWith rdf:resource="http://www.openmath.org/ontology#CDBase"/>
    <rdfs:comment>The status of a CD, as described in sections 4.2.1 and 4.3.2</rdfs:comment>
    <owl:oneOf rdf:nodeID="A51"/>
    <rdfs:isDefinedBy rdf:resource="http://www.openmath.org/ontology#"/>
  </rdf:Description>
  <rdf:Description rdf:nodeID="A2">
    <rdf:first rdf:resource="http://www.openmath.org/ontology#ContentDictionary"/>
    <rdf:rest rdf:nodeID="A44"/>
  </rdf:Description>
  <rdf:Description rdf:about="http://www.openmath.org/ontology#hasText">
    <rdf:type rdf:resource="http://www.w3.org/2002/07/owl#DatatypeProperty"/>
    <rdfs:domain rdf:nodeID="A6"/>
    <rdfs:range rdf:resource="http://www.w3.org/2000/01/rdf-schema#Literal"/>
    <rdfs:comment>The text of a property (usually an informal one)</rdfs:comment>
    <rdfs:isDefinedBy rdf:resource="http://www.openmath.org/ontology#"/>
  </rdf:Description>
  <rdf:Description rdf:nodeID="A19">
    <rdf:type rdf:resource="http://www.w3.org/2002/07/owl#Restriction"/>
    <owl:onProperty rdf:resource="http://www.openmath.org/ontology#minor"/>
    <owl:allValuesFrom rdf:resource="http://www.w3.org/2001/XMLSchema#nonNegativeInteger"/>
  </rdf:Description>
  <rdf:Description rdf:nodeID="A43">
    <rdf:first rdf:resource="http://www.openmath.org/ontology#hasFormalPart"/>
    <rdf:rest rdf:nodeID="A28"/>
  </rdf:Description>
  <rdf:Description rdf:about="http://www.openmath.org/ontology#Official">
    <rdf:type rdf:resource="http://www.openmath.org/ontology#Status"/>
    <rdfs:comment>The 'official' status of a CD, as described in section 4.2.1</rdfs:comment>
    <rdfs:isDefinedBy rdf:resource="http://www.openmath.org/ontology#"/>
  </rdf:Description>
  <rdf:Description rdf:nodeID="A51">
    <rdf:first rdf:resource="http://www.openmath.org/ontology#Official"/>
    <rdf:rest rdf:nodeID="A46"/>
  </rdf:Description>
  <rdf:Description rdf:about="http://www.openmath.org/ontology#CommentedPart">
    <rdf:type rdf:resource="http://www.w3.org/2002/07/owl#Class"/>
    <rdfs:subClassOf rdf:resource="http://www.openmath.org/ontology#OpenMathConcept"/>
    <owl:disjointWith rdf:resource="http://www.openmath.org/ontology#Composite"/>
    <owl:disjointWith rdf:resource="http://www.openmath.org/ontology#CDBase"/>
    <owl:disjointWith rdf:resource="http://www.openmath.org/ontology#Status"/>
    <owl:disjointWith rdf:resource="http://www.openmath.org/ontology#Role"/>
    <rdfs:comment>A commented part of a mathematical property (CMP) of a symbol, as described in sections 4.2 and 4.3</rdfs:comment>
    <rdfs:isDefinedBy rdf:resource="http://www.openmath.org/ontology#"/>
  </rdf:Description>
  <rdf:Description rdf:nodeID="A47">
    <rdf:first rdf:resource="http://www.openmath.org/ontology#Private"/>
    <rdf:rest rdf:nodeID="A8"/>
  </rdf:Description>
  <rdf:Description rdf:nodeID="A45">
    <rdf:first rdf:resource="http://www.openmath.org/ontology#FormalPart"/>
    <rdf:rest rdf:nodeID="A5"/>
  </rdf:Description>
  <rdf:Description rdf:nodeID="A49">
    <rdf:type rdf:resource="http://www.w3.org/2002/07/owl#Restriction"/>
    <owl:onProperty rdf:resource="http://purl.org/dc/terms/identifier"/>
    <owl:cardinality rdf:datatype="http://www.w3.org/2001/XMLSchema#nonNegativeInteger">1</owl:cardinality>
  </rdf:Description>
  <rdf:Description rdf:nodeID="A21">
    <rdf:type rdf:resource="http://www.w3.org/2002/07/owl#Restriction"/>
    <owl:onProperty rdf:resource="http://www.openmath.org/ontology#major"/>
    <owl:allValuesFrom rdf:resource="http://www.w3.org/2001/XMLSchema#nonNegativeInteger"/>
  </rdf:Description>
</rdf:RDF>
