<rdf:RDF
    xmlns:rdf="http://www.w3.org/1999/02/22-rdf-syntax-ns#"
    xmlns:cd="http://www.openmath.org/cd/"
    xmlns:oo="http://omdoc.org/ontology#"
    xmlns:owl="http://www.w3.org/2002/07/owl#"
    xmlns:dct="http://purl.org/dc/terms/"
    xmlns:xsd="http://www.w3.org/2001/XMLSchema#"
    xmlns:omo="http://www.openmath.org/ontology#"
    xmlns:rdfs="http://www.w3.org/2000/01/rdf-schema#" > 
  <rdf:Description rdf:about="http://www.openmath.org/ontology#type">
    <rdf:type rdf:resource="http://www.w3.org/2002/07/owl#ObjectProperty"/>
    <rdf:type rdf:resource="http://www.w3.org/2002/07/owl#InverseFunctionalProperty"/>
    <owl:inverseOf rdf:resource="http://www.openmath.org/ontology#typesSymbol"/>
    <rdfs:label xml:lang="en">type</rdfs:label>
    <rdfs:isDefinedBy rdf:resource="http://www.openmath.org/ontology#"/>
  </rdf:Description>
  <rdf:Description rdf:nodeID="A0">
    <rdf:first rdf:resource="http://www.openmath.org/ontology#exemplifiedBy"/>
    <rdf:rest rdf:nodeID="A1"/>
  </rdf:Description>
  <rdf:Description rdf:about="http://www.openmath.org/ontology#hasDirectPart">
    <rdf:type rdf:resource="http://www.w3.org/2002/07/owl#InverseFunctionalProperty"/>
    <rdf:type rdf:resource="http://www.w3.org/2002/07/owl#ObjectProperty"/>
    <rdfs:subPropertyOf rdf:resource="http://www.openmath.org/ontology#hasPart"/>
    <rdfs:comment>This relation denotes that one concept A directly logically contains another concept B, and that B is not contained by any other concept than A, as reflected by child elements in OpenMath XML documents.</rdfs:comment>
    <rdfs:label xml:lang="en">has direct part</rdfs:label>
    <rdfs:isDefinedBy rdf:resource="http://www.openmath.org/ontology#"/>
  </rdf:Description>
  <rdf:Description rdf:about="http://purl.org/dc/terms/identifier">
    <rdf:type rdf:resource="http://www.w3.org/2002/07/owl#DatatypeProperty"/>
  </rdf:Description>
  <rdf:Description rdf:about="http://www.openmath.org/ontology#reviewDate">
    <rdf:type rdf:resource="http://www.w3.org/2002/07/owl#DatatypeProperty"/>
    <rdf:type rdf:resource="http://www.w3.org/2002/07/owl#FunctionalProperty"/>
    <rdfs:domain rdf:resource="http://www.openmath.org/ontology#Dictionary"/>
    <rdfs:range rdf:resource="http://www.w3.org/2001/XMLSchema#date"/>
    <rdfs:comment>The review date of a content dictionary or signature dictionary, as described in section 4.2 and 4.3.2</rdfs:comment>
    <rdfs:label xml:lang="en">review date</rdfs:label>
    <rdfs:isDefinedBy rdf:resource="http://www.openmath.org/ontology#"/>
  </rdf:Description>
  <rdf:Description rdf:about="http://www.openmath.org/ontology#Private">
    <rdf:type rdf:resource="http://www.openmath.org/ontology#Status"/>
    <rdfs:comment>The 'private' status of a CD, as described in section 4.2.1</rdfs:comment>
    <rdfs:label xml:lang="en">private</rdfs:label>
    <rdfs:isDefinedBy rdf:resource="http://www.openmath.org/ontology#"/>
  </rdf:Description>
  <rdf:Description rdf:nodeID="A2">
    <owl:unionOf rdf:nodeID="A3"/>
  </rdf:Description>
  <rdf:Description rdf:nodeID="A4">
    <rdf:type rdf:resource="http://www.w3.org/2002/07/owl#Restriction"/>
    <owl:onProperty rdf:resource="http://purl.org/dc/terms/description"/>
    <owl:cardinality rdf:datatype="http://www.w3.org/2001/XMLSchema#nonNegativeInteger">1</owl:cardinality>
  </rdf:Description>
  <rdf:Description rdf:about="http://www.openmath.org/ontology#hasCommentedPart">
    <rdf:type rdf:resource="http://www.w3.org/2002/07/owl#ObjectProperty"/>
    <rdf:type rdf:resource="http://www.w3.org/2002/07/owl#FunctionalProperty"/>
    <rdfs:subPropertyOf rdf:resource="http://www.openmath.org/ontology#hasDirectPart"/>
    <rdfs:domain rdf:resource="http://www.openmath.org/ontology#Property"/>
    <rdfs:range rdf:resource="http://www.openmath.org/ontology#CommentedPart"/>
    <rdfs:comment>The relationship of a property container to its commented part (CMP).</rdfs:comment>
    <rdfs:label xml:lang="en">commented part</rdfs:label>
    <rdfs:isDefinedBy rdf:resource="http://www.openmath.org/ontology#"/>
  </rdf:Description>
  <rdf:Description rdf:about="http://www.openmath.org/ontology#">
    <rdf:type rdf:resource="http://www.w3.org/2002/07/owl#Ontology"/>
    <dct:title>OpenMath 2.0/3.0 content dictionary ontology</dct:title>
    <rdfs:comment>OpenMath 2.0/3.0 content dictionary ontology in OWL-DL, modeled after the OpenMath 2.0 specification and currently in transition towards OpenMath 3.0.  All references to chapters and sections point to the OpenMath 2.0 standard.</rdfs:comment>
    <dct:creator>Christoph Lange &lt;ch.lange@jacobs-university.de&gt;</dct:creator>
    <dct:subject>Semantic Mathematical Markup</dct:subject>
    <owl:versionInfo>0.3.2</owl:versionInfo>
    <owl:imports rdf:resource="http://omdoc.org/ontology#"/>
  </rdf:Description>
  <rdf:Description rdf:about="http://www.openmath.org/ontology#OpenMathConcept">
    <rdf:type rdf:resource="http://www.w3.org/2002/07/owl#Class"/>
    <rdfs:subClassOf rdf:resource="http://omdoc.org/ontology#MathKnowledgeItem"/>
    <rdfs:comment>The generic superclass of all concepts that can be expressed in OpenMath content/signature/notation dictionaries</rdfs:comment>
    <rdfs:label xml:lang="en">OpenMath concept</rdfs:label>
    <rdfs:isDefinedBy rdf:resource="http://www.openmath.org/ontology#"/>
  </rdf:Description>
  <rdf:Description rdf:nodeID="A5">
    <rdf:first rdf:resource="http://www.openmath.org/ontology#ContentDictionary"/>
    <rdf:rest rdf:nodeID="A6"/>
  </rdf:Description>
  <rdf:Description rdf:about="http://www.openmath.org/ontology#SemanticAttribution">
    <rdf:type rdf:resource="http://www.openmath.org/ontology#Role"/>
    <rdfs:comment>The 'semantic attribution' role of a symbol, as described in section 2.1.4</rdfs:comment>
    <rdfs:label xml:lang="en">semantic attribution</rdfs:label>
    <rdfs:isDefinedBy rdf:resource="http://www.openmath.org/ontology#"/>
  </rdf:Description>
  <rdf:Description rdf:about="http://www.openmath.org/ontology#NotationDefinition">
    <rdf:type rdf:resource="http://www.w3.org/2002/07/owl#Class"/>
    <owl:disjointWith rdf:resource="http://www.openmath.org/ontology#FormalPart"/>
    <owl:disjointWith rdf:resource="http://www.openmath.org/ontology#Role"/>
    <owl:disjointWith rdf:resource="http://www.openmath.org/ontology#Signature"/>
    <owl:disjointWith rdf:resource="http://www.openmath.org/ontology#Status"/>
    <owl:disjointWith rdf:resource="http://www.openmath.org/ontology#CommentedPart"/>
    <owl:disjointWith rdf:resource="http://www.openmath.org/ontology#Example"/>
    <rdfs:label xml:lang="en">notation definition</rdfs:label>
    <rdfs:isDefinedBy rdf:resource="http://www.openmath.org/ontology#"/>
    <owl:disjointWith rdf:resource="http://www.openmath.org/ontology#CDBase"/>
    <rdfs:subClassOf rdf:resource="http://www.openmath.org/ontology#OpenMathConcept"/>
    <rdfs:comment>A notation definition for one symbol</rdfs:comment>
    <owl:disjointWith rdf:resource="http://www.openmath.org/ontology#Composite"/>
  </rdf:Description>
  <rdf:Description rdf:nodeID="A7">
    <rdf:type rdf:resource="http://www.w3.org/2002/07/owl#Restriction"/>
    <owl:onProperty rdf:resource="http://purl.org/dc/terms/description"/>
    <owl:cardinality rdf:datatype="http://www.w3.org/2001/XMLSchema#nonNegativeInteger">1</owl:cardinality>
  </rdf:Description>
  <rdf:Description rdf:about="http://www.openmath.org/ontology#Obsolete">
    <rdf:type rdf:resource="http://www.openmath.org/ontology#Status"/>
    <rdfs:comment>The 'obsolete' status of a CD, as described in section 4.2.1</rdfs:comment>
    <rdfs:label xml:lang="en">obsolete</rdfs:label>
    <rdfs:isDefinedBy rdf:resource="http://www.openmath.org/ontology#"/>
  </rdf:Description>
  <rdf:Description rdf:about="http://www.openmath.org/ontology#comprises">
    <rdf:type rdf:resource="http://www.w3.org/2002/07/owl#ObjectProperty"/>
    <rdf:type rdf:resource="http://www.w3.org/2002/07/owl#TransitiveProperty"/>
    <rdfs:domain rdf:resource="http://www.openmath.org/ontology#Composite"/>
    <rdfs:range rdf:resource="http://www.openmath.org/ontology#OpenMathConcept"/>
    <rdfs:comment>This relation denotes that one concept A directly or indirectly comprises another concept B, but does not necessarily exclusively contain it.</rdfs:comment>
    <rdfs:label xml:lang="en">comprises</rdfs:label>
    <rdfs:isDefinedBy rdf:resource="http://www.openmath.org/ontology#"/>
  </rdf:Description>
  <rdf:Description rdf:about="http://www.openmath.org/ontology#hasNotationDictionary">
    <rdf:type rdf:resource="http://www.w3.org/2002/07/owl#ObjectProperty"/>
    <rdf:type rdf:resource="http://www.w3.org/2002/07/owl#InverseFunctionalProperty"/>
    <owl:inverseOf rdf:resource="http://www.openmath.org/ontology#containsNotationsFor"/>
    <rdfs:isDefinedBy rdf:resource="http://www.openmath.org/ontology#"/>
  </rdf:Description>
  <rdf:Description rdf:nodeID="A1">
    <rdf:first rdf:resource="http://www.openmath.org/ontology#usesSymbol"/>
    <rdf:rest rdf:nodeID="A8"/>
  </rdf:Description>
  <rdf:Description rdf:about="http://www.openmath.org/ontology#Experimental">
    <rdf:type rdf:resource="http://www.openmath.org/ontology#Status"/>
    <rdfs:comment>The 'experimental' status of a CD, as described in section 4.2.1</rdfs:comment>
    <rdfs:label xml:lang="en">experimental</rdfs:label>
    <rdfs:isDefinedBy rdf:resource="http://www.openmath.org/ontology#"/>
  </rdf:Description>
  <rdf:Description rdf:about="http://www.openmath.org/ontology#typeSystem">
    <rdf:type rdf:resource="http://www.w3.org/2002/07/owl#ObjectProperty"/>
    <rdf:type rdf:resource="http://www.w3.org/2002/07/owl#FunctionalProperty"/>
    <rdfs:domain rdf:resource="http://www.openmath.org/ontology#SignatureDictionary"/>
    <rdfs:range rdf:nodeID="A9"/>
    <rdfs:comment>The content dictionary [group] that serves as a type system for this signature dictionary, as specified in section 4.4.1.1</rdfs:comment>
    <rdfs:label xml:lang="en">type system</rdfs:label>
    <rdfs:isDefinedBy rdf:resource="http://www.openmath.org/ontology#"/>
  </rdf:Description>
  <rdf:Description rdf:about="http://www.openmath.org/ontology#SymbolDefinition">
    <rdfs:subClassOf rdf:nodeID="A7"/>
    <owl:disjointWith rdf:resource="http://www.openmath.org/ontology#ContentDictionaryGroup"/>
    <rdfs:subClassOf rdf:resource="http://www.openmath.org/ontology#Composite"/>
    <rdfs:comment>An OpenMath symbol definition, as described in section 4.2SD and 4.3.  Some of the properties of symbols are defined as properties in this ontology, others are taken from Dublin Core and RDFS, with the following mapping: Name = dct:identifier, Title = dct:title, CDComment = rdfs:comment.</rdfs:comment>
    <rdfs:label xml:lang="en">symbol definition</rdfs:label>
    <rdfs:subClassOf rdf:nodeID="A10"/>
    <rdf:type rdf:resource="http://www.w3.org/2002/07/owl#Class"/>
    <owl:disjointWith rdf:resource="http://www.openmath.org/ontology#Dictionary"/>
    <rdfs:subClassOf rdf:nodeID="A11"/>
    <rdfs:comment>OpenMath 2+/3 transitional aspects: Title = dct:title</rdfs:comment>
    <rdfs:isDefinedBy rdf:resource="http://www.openmath.org/ontology#"/>
  </rdf:Description>
  <rdf:Description rdf:nodeID="A12">
    <rdf:type rdf:resource="http://www.w3.org/2002/07/owl#Restriction"/>
    <owl:onProperty rdf:resource="http://purl.org/dc/terms/date"/>
    <owl:cardinality rdf:datatype="http://www.w3.org/2001/XMLSchema#nonNegativeInteger">1</owl:cardinality>
  </rdf:Description>
  <rdf:Description rdf:about="http://purl.org/dc/terms/creator">
    <rdf:type rdf:resource="http://www.w3.org/2002/07/owl#AnnotationProperty"/>
  </rdf:Description>
  <rdf:Description rdf:nodeID="A13">
    <rdf:first rdf:resource="http://www.openmath.org/ontology#definedIn"/>
    <rdf:rest rdf:resource="http://www.w3.org/1999/02/22-rdf-syntax-ns#nil"/>
  </rdf:Description>
  <rdf:Description rdf:about="http://www.openmath.org/ontology#usesSymbol">
    <rdf:type rdf:resource="http://www.w3.org/2002/07/owl#ObjectProperty"/>
    <rdfs:domain rdf:nodeID="A14"/>
    <rdfs:range rdf:resource="http://www.openmath.org/ontology#SymbolDefinition"/>
    <rdfs:comment>The relationship of some element to a symbol used in an OpenMath object inside the element</rdfs:comment>
    <rdfs:label xml:lang="en">uses</rdfs:label>
    <rdfs:isDefinedBy rdf:resource="http://www.openmath.org/ontology#"/>
  </rdf:Description>
  <rdf:Description rdf:about="http://www.openmath.org/ontology#Dictionary">
    <rdf:type rdf:resource="http://www.w3.org/2002/07/owl#Class"/>
    <rdfs:subClassOf rdf:resource="http://www.openmath.org/ontology#Composite"/>
    <rdfs:label xml:lang="en">dictionary</rdfs:label>
    <owl:disjointWith rdf:resource="http://www.openmath.org/ontology#ContentDictionaryGroup"/>
    <rdfs:isDefinedBy rdf:resource="http://www.openmath.org/ontology#"/>
  </rdf:Description>
  <rdf:Description rdf:about="http://www.openmath.org/ontology#url">
    <rdf:type rdf:resource="http://www.w3.org/2002/07/owl#ObjectProperty"/>
    <rdf:type rdf:resource="http://www.w3.org/2002/07/owl#FunctionalProperty"/>
    <rdfs:domain rdf:nodeID="A2"/>
    <rdfs:comment>The URL of a content dictionary or content dictionary group, as described in section 4.3.2 or 4.4.2.2, resp.</rdfs:comment>
    <rdfs:label xml:lang="en">URL</rdfs:label>
    <rdfs:isDefinedBy rdf:resource="http://www.openmath.org/ontology#"/>
  </rdf:Description>
  <rdf:Description rdf:about="http://www.openmath.org/ontology#hasNotationDefinition">
    <rdf:type rdf:resource="http://www.w3.org/2002/07/owl#ObjectProperty"/>
    <rdf:type rdf:resource="http://www.w3.org/2002/07/owl#InverseFunctionalProperty"/>
    <owl:inverseOf rdf:resource="http://www.openmath.org/ontology#rendersSymbol"/>
    <rdfs:label xml:lang="en">notation definition</rdfs:label>
    <rdfs:isDefinedBy rdf:resource="http://www.openmath.org/ontology#"/>
  </rdf:Description>
  <rdf:Description rdf:nodeID="A6">
    <rdf:first rdf:resource="http://www.openmath.org/ontology#ContentDictionaryGroup"/>
    <rdf:rest rdf:resource="http://www.w3.org/1999/02/22-rdf-syntax-ns#nil"/>
  </rdf:Description>
  <rdf:Description rdf:nodeID="A10">
    <rdf:type rdf:resource="http://www.w3.org/2002/07/owl#Restriction"/>
    <owl:onProperty rdf:resource="http://purl.org/dc/terms/identifier"/>
    <owl:allValuesFrom rdf:resource="http://www.w3.org/2001/XMLSchema#NCName"/>
  </rdf:Description>
  <rdf:Description rdf:about="http://www.openmath.org/ontology#Binder">
    <rdf:type rdf:resource="http://www.openmath.org/ontology#Role"/>
    <rdfs:comment>The 'binder' role of a symbol, as described in section 2.1.4</rdfs:comment>
    <rdfs:label xml:lang="en">binder</rdfs:label>
    <rdfs:isDefinedBy rdf:resource="http://www.openmath.org/ontology#"/>
  </rdf:Description>
  <rdf:Description rdf:about="http://www.openmath.org/ontology#Attribution">
    <rdf:type rdf:resource="http://www.openmath.org/ontology#Role"/>
    <rdfs:comment>The 'attribution' role of a symbol, as described in section 2.1.4</rdfs:comment>
    <rdfs:label xml:lang="en">attribution</rdfs:label>
    <rdfs:isDefinedBy rdf:resource="http://www.openmath.org/ontology#"/>
  </rdf:Description>
  <rdf:Description rdf:about="http://www.openmath.org/ontology#hasFormalPart">
    <rdf:type rdf:resource="http://www.w3.org/2002/07/owl#ObjectProperty"/>
    <rdf:type rdf:resource="http://www.w3.org/2002/07/owl#FunctionalProperty"/>
    <rdfs:subPropertyOf rdf:resource="http://www.openmath.org/ontology#hasDirectPart"/>
    <rdfs:domain rdf:resource="http://www.openmath.org/ontology#Property"/>
    <rdfs:range rdf:resource="http://www.openmath.org/ontology#FormalPart"/>
    <rdfs:comment>The relationship of a property container to its formal part (FMP).</rdfs:comment>
    <rdfs:label xml:lang="en">formal part</rdfs:label>
    <rdfs:isDefinedBy rdf:resource="http://www.openmath.org/ontology#"/>
  </rdf:Description>
  <rdf:Description rdf:nodeID="A8">
    <rdf:first rdf:resource="http://www.openmath.org/ontology#definedIn"/>
    <rdf:rest rdf:resource="http://www.w3.org/1999/02/22-rdf-syntax-ns#nil"/>
  </rdf:Description>
  <rdf:Description rdf:about="http://purl.org/dc/terms/description">
    <rdf:type rdf:resource="http://www.w3.org/2002/07/owl#DatatypeProperty"/>
  </rdf:Description>
  <rdf:Description rdf:about="http://www.openmath.org/ontology#Version">
    <rdfs:label xml:lang="en">version</rdfs:label>
    <owl:disjointWith rdf:resource="http://www.openmath.org/ontology#Example"/>
    <owl:disjointWith rdf:resource="http://www.openmath.org/ontology#NotationDefinition"/>
    <rdfs:isDefinedBy rdf:resource="http://www.openmath.org/ontology#"/>
    <owl:disjointWith rdf:resource="http://www.openmath.org/ontology#FormalPart"/>
    <owl:disjointWith rdf:resource="http://www.openmath.org/ontology#CommentedPart"/>
    <owl:disjointWith rdf:resource="http://www.openmath.org/ontology#Status"/>
    <owl:disjointWith rdf:resource="http://www.openmath.org/ontology#Role"/>
    <rdfs:subClassOf rdf:nodeID="A15"/>
    <rdfs:subClassOf rdf:nodeID="A16"/>
    <rdf:type rdf:resource="http://www.w3.org/2002/07/owl#Class"/>
    <owl:disjointWith rdf:resource="http://www.openmath.org/ontology#Composite"/>
    <owl:disjointWith rdf:resource="http://www.openmath.org/ontology#CDBase"/>
    <rdfs:subClassOf rdf:resource="http://www.openmath.org/ontology#OpenMathConcept"/>
    <rdfs:comment>A version with major and minor part (both mandatory), as described in section 4.2, 4.3.2 or 4.4.2.2, resp.</rdfs:comment>
    <rdfs:subClassOf rdf:nodeID="A17"/>
    <rdfs:subClassOf rdf:nodeID="A18"/>
    <owl:disjointWith rdf:resource="http://www.openmath.org/ontology#Signature"/>
  </rdf:Description>
  <rdf:Description rdf:about="http://www.openmath.org/ontology#hasSignatureDictionary">
    <rdf:type rdf:resource="http://www.w3.org/2002/07/owl#ObjectProperty"/>
    <rdf:type rdf:resource="http://www.w3.org/2002/07/owl#InverseFunctionalProperty"/>
    <owl:inverseOf rdf:resource="http://www.openmath.org/ontology#containsSignaturesFor"/>
    <rdfs:label xml:lang="en">signature dictionary</rdfs:label>
    <rdfs:isDefinedBy rdf:resource="http://www.openmath.org/ontology#"/>
  </rdf:Description>
  <rdf:Description rdf:about="http://www.openmath.org/ontology#FormalPart">
    <owl:disjointWith rdf:resource="http://www.openmath.org/ontology#Role"/>
    <rdfs:isDefinedBy rdf:resource="http://www.openmath.org/ontology#"/>
    <rdfs:label xml:lang="en">formal part</rdfs:label>
    <owl:disjointWith rdf:resource="http://www.openmath.org/ontology#Composite"/>
    <owl:disjointWith rdf:resource="http://www.openmath.org/ontology#CDBase"/>
    <rdf:type rdf:resource="http://www.w3.org/2002/07/owl#Class"/>
    <owl:disjointWith rdf:resource="http://www.openmath.org/ontology#Status"/>
    <owl:disjointWith rdf:resource="http://www.openmath.org/ontology#CommentedPart"/>
    <rdfs:subClassOf rdf:resource="http://www.openmath.org/ontology#OpenMathConcept"/>
    <rdfs:comment>A formal part of a mathematical property (FMP) of a symbol, as described in sections 4.2 and 4.3</rdfs:comment>
  </rdf:Description>
  <rdf:Description rdf:nodeID="A19">
    <rdf:first rdf:resource="http://www.openmath.org/ontology#ContentDictionaryGroup"/>
    <rdf:rest rdf:resource="http://www.w3.org/1999/02/22-rdf-syntax-ns#nil"/>
  </rdf:Description>
  <rdf:Description rdf:nodeID="A20">
    <rdf:type rdf:resource="http://www.w3.org/2002/07/owl#Restriction"/>
    <owl:onProperty rdf:resource="http://purl.org/dc/terms/date"/>
    <owl:allValuesFrom rdf:resource="http://www.w3.org/2001/XMLSchema#date"/>
  </rdf:Description>
  <rdf:Description rdf:about="http://www.openmath.org/ontology#exemplifies">
    <rdf:type rdf:resource="http://www.w3.org/2002/07/owl#ObjectProperty"/>
    <rdf:type rdf:resource="http://www.w3.org/2002/07/owl#FunctionalProperty"/>
    <owl:inverseOf rdf:resource="http://www.openmath.org/ontology#exemplifiedBy"/>
    <rdfs:label xml:lang="en">exemplifies</rdfs:label>
    <rdfs:isDefinedBy rdf:resource="http://www.openmath.org/ontology#"/>
  </rdf:Description>
  <rdf:Description rdf:about="http://www.openmath.org/ontology#hasPragmaticSyntax">
    <rdf:type rdf:resource="http://www.w3.org/2002/07/owl#ObjectProperty"/>
    <rdfs:subPropertyOf rdf:resource="http://www.openmath.org/ontology#hasDirectPart"/>
    <rdfs:comment>OpenMath 2+/3 transitional</rdfs:comment>
    <rdfs:domain rdf:resource="http://www.openmath.org/ontology#SymbolDefinition"/>
    <rdfs:range rdf:resource="http://www.openmath.org/ontology#PragmaticSyntax"/>
    <rdfs:comment>The relationship of a symbol definition to its pragmatic usage guidelines</rdfs:comment>
    <rdfs:label xml:lang="en">pragmatic syntax</rdfs:label>
    <rdfs:isDefinedBy rdf:resource="http://www.openmath.org/ontology#"/>
  </rdf:Description>
  <rdf:Description rdf:about="http://www.openmath.org/ontology#usesDirectly">
    <rdf:type rdf:resource="http://www.w3.org/2002/07/owl#ObjectProperty"/>
    <rdfs:subPropertyOf rdf:resource="http://www.openmath.org/ontology#uses"/>
    <rdfs:domain rdf:resource="http://www.openmath.org/ontology#ContentDictionary"/>
    <rdfs:range rdf:resource="http://www.openmath.org/ontology#ContentDictionary"/>
    <owl:propertyChainAxiom rdf:nodeID="A21"/>
    <owl:propertyChainAxiom rdf:nodeID="A22"/>
    <rdfs:comment>Other content dictionaries directly used by this one, as described in section 4.3.2</rdfs:comment>
    <rdfs:label xml:lang="en">uses directly</rdfs:label>
    <rdfs:isDefinedBy rdf:resource="http://www.openmath.org/ontology#"/>
  </rdf:Description>
  <rdf:Description rdf:about="http://www.openmath.org/ontology#Property">
    <rdf:type rdf:resource="http://www.w3.org/2002/07/owl#Class"/>
    <rdfs:subClassOf rdf:resource="http://www.openmath.org/ontology#Composite"/>
    <owl:disjointWith rdf:resource="http://www.openmath.org/ontology#ContentDictionaryGroup"/>
    <owl:disjointWith rdf:resource="http://www.openmath.org/ontology#Dictionary"/>
    <owl:disjointWith rdf:resource="http://www.openmath.org/ontology#SymbolDefinition"/>
    <rdfs:comment>A mathematical property of a symbol, can have a commented (CMP), a formal (FMP) part, or both; cf. sections 4.2 and 4.3</rdfs:comment>
    <rdfs:label xml:lang="en">mathematical property</rdfs:label>
    <rdfs:isDefinedBy rdf:resource="http://www.openmath.org/ontology#"/>
  </rdf:Description>
  <rdf:Description rdf:nodeID="A15">
    <rdf:type rdf:resource="http://www.w3.org/2002/07/owl#Restriction"/>
    <owl:onProperty rdf:resource="http://www.openmath.org/ontology#major"/>
    <owl:cardinality rdf:datatype="http://www.w3.org/2001/XMLSchema#nonNegativeInteger">1</owl:cardinality>
  </rdf:Description>
  <rdf:Description rdf:about="http://www.openmath.org/ontology#containsContentDictionary">
    <rdf:type rdf:resource="http://www.w3.org/2002/07/owl#ObjectProperty"/>
    <rdfs:subPropertyOf rdf:resource="http://www.openmath.org/ontology#comprises"/>
    <rdfs:domain rdf:resource="http://www.openmath.org/ontology#ContentDictionaryGroup"/>
    <rdfs:range rdf:resource="http://www.openmath.org/ontology#ContentDictionary"/>
    <rdfs:comment>The relationship of a content dictionary group to a content dictionary it contains</rdfs:comment>
    <rdfs:label xml:lang="en">contains CD</rdfs:label>
    <rdfs:isDefinedBy rdf:resource="http://www.openmath.org/ontology#"/>
  </rdf:Description>
  <rdf:Description rdf:nodeID="A21">
    <rdf:first rdf:resource="http://www.openmath.org/ontology#definesSymbol"/>
    <rdf:rest rdf:nodeID="A23"/>
  </rdf:Description>
  <rdf:Description rdf:nodeID="A11">
    <rdf:type rdf:resource="http://www.w3.org/2002/07/owl#Restriction"/>
    <owl:onProperty rdf:resource="http://purl.org/dc/terms/identifier"/>
    <owl:cardinality rdf:datatype="http://www.w3.org/2001/XMLSchema#nonNegativeInteger">1</owl:cardinality>
  </rdf:Description>
  <rdf:Description rdf:about="http://www.openmath.org/ontology#definesSymbol">
    <rdf:type rdf:resource="http://www.w3.org/2002/07/owl#ObjectProperty"/>
    <rdfs:subPropertyOf rdf:resource="http://www.openmath.org/ontology#hasDirectPart"/>
    <rdfs:domain rdf:resource="http://www.openmath.org/ontology#ContentDictionary"/>
    <rdfs:range rdf:resource="http://www.openmath.org/ontology#SymbolDefinition"/>
    <owl:inverseOf rdf:resource="http://www.openmath.org/ontology#definedIn"/>
    <rdfs:comment>The relationship of a content dictionary to a symbol it defines</rdfs:comment>
    <rdfs:label xml:lang="en">defines</rdfs:label>
    <rdfs:isDefinedBy rdf:resource="http://www.openmath.org/ontology#"/>
  </rdf:Description>
  <rdf:Description rdf:about="http://purl.org/dc/terms/subject">
    <rdf:type rdf:resource="http://www.w3.org/2002/07/owl#AnnotationProperty"/>
  </rdf:Description>
  <rdf:Description rdf:nodeID="A24">
    <rdf:type rdf:resource="http://www.w3.org/2002/07/owl#Restriction"/>
    <owl:onProperty rdf:resource="http://www.openmath.org/ontology#status"/>
    <owl:cardinality rdf:datatype="http://www.w3.org/2001/XMLSchema#nonNegativeInteger">1</owl:cardinality>
  </rdf:Description>
  <rdf:Description rdf:about="http://www.openmath.org/ontology#uses">
    <rdf:type rdf:resource="http://www.w3.org/2002/07/owl#ObjectProperty"/>
    <rdf:type rdf:resource="http://www.w3.org/2002/07/owl#TransitiveProperty"/>
    <rdfs:subPropertyOf rdf:resource="http://omdoc.org/ontology#dependsOn"/>
    <rdfs:label xml:lang="en">uses</rdfs:label>
    <rdfs:isDefinedBy rdf:resource="http://www.openmath.org/ontology#"/>
  </rdf:Description>
  <rdf:Description rdf:nodeID="A25">
    <rdf:type rdf:resource="http://www.w3.org/2002/07/owl#Restriction"/>
    <owl:onProperty rdf:resource="http://purl.org/dc/terms/identifier"/>
    <owl:cardinality rdf:datatype="http://www.w3.org/2001/XMLSchema#nonNegativeInteger">1</owl:cardinality>
  </rdf:Description>
  <rdf:Description rdf:about="http://www.openmath.org/ontology#status">
    <rdf:type rdf:resource="http://www.w3.org/2002/07/owl#ObjectProperty"/>
    <rdf:type rdf:resource="http://www.w3.org/2002/07/owl#FunctionalProperty"/>
    <rdfs:domain rdf:resource="http://www.openmath.org/ontology#Dictionary"/>
    <rdfs:range rdf:resource="http://www.openmath.org/ontology#Status"/>
    <rdfs:comment>The status of a content dictionary or signature dictionary, as described in section 4.2.1 and 4.3.2</rdfs:comment>
    <rdfs:label xml:lang="en">status</rdfs:label>
    <rdfs:isDefinedBy rdf:resource="http://www.openmath.org/ontology#"/>
  </rdf:Description>
  <rdf:Description rdf:nodeID="A3">
    <rdf:first rdf:resource="http://www.openmath.org/ontology#ContentDictionary"/>
    <rdf:rest rdf:nodeID="A19"/>
  </rdf:Description>
  <rdf:Description rdf:about="http://www.openmath.org/ontology#minor">
    <rdf:type rdf:resource="http://www.w3.org/2002/07/owl#DatatypeProperty"/>
    <rdf:type rdf:resource="http://www.w3.org/2002/07/owl#FunctionalProperty"/>
    <rdfs:domain rdf:resource="http://www.openmath.org/ontology#Version"/>
    <rdfs:range rdf:resource="http://www.w3.org/2001/XMLSchema#nonNegativeInteger"/>
    <rdfs:comment>Minor part of a version number, as described in section 4.2.2</rdfs:comment>
    <rdfs:label xml:lang="en">minor part</rdfs:label>
    <rdfs:isDefinedBy rdf:resource="http://www.openmath.org/ontology#"/>
  </rdf:Description>
  <rdf:Description rdf:nodeID="A26">
    <rdf:type rdf:resource="http://www.w3.org/2002/07/owl#Restriction"/>
    <owl:onProperty rdf:resource="http://www.openmath.org/ontology#reviewDate"/>
    <owl:cardinality rdf:datatype="http://www.w3.org/2001/XMLSchema#nonNegativeInteger">1</owl:cardinality>
  </rdf:Description>
  <rdf:Description rdf:about="http://www.openmath.org/ontology#Example">
    <owl:disjointWith rdf:resource="http://www.openmath.org/ontology#Composite"/>
    <rdfs:subClassOf rdf:resource="http://www.openmath.org/ontology#OpenMathConcept"/>
    <owl:disjointWith rdf:resource="http://www.openmath.org/ontology#Role"/>
    <rdf:type rdf:resource="http://www.w3.org/2002/07/owl#Class"/>
    <rdfs:comment>An example for a symbol, as described in sections 4.2 and 4.3</rdfs:comment>
    <owl:disjointWith rdf:resource="http://www.openmath.org/ontology#Status"/>
    <rdfs:isDefinedBy rdf:resource="http://www.openmath.org/ontology#"/>
    <rdfs:label xml:lang="en">example</rdfs:label>
    <owl:disjointWith rdf:resource="http://www.openmath.org/ontology#CDBase"/>
    <owl:disjointWith rdf:resource="http://www.openmath.org/ontology#FormalPart"/>
    <owl:disjointWith rdf:resource="http://www.openmath.org/ontology#CommentedPart"/>
  </rdf:Description>
  <rdf:Description rdf:nodeID="A27">
    <owl:unionOf rdf:nodeID="A5"/>
  </rdf:Description>
  <rdf:Description rdf:about="http://www.openmath.org/ontology#Constant">
    <rdf:type rdf:resource="http://www.openmath.org/ontology#Role"/>
    <rdfs:comment>The 'constant' role of a symbol, as described in section 2.1.4</rdfs:comment>
    <rdfs:label xml:lang="en">constant</rdfs:label>
    <rdfs:isDefinedBy rdf:resource="http://www.openmath.org/ontology#"/>
  </rdf:Description>
  <rdf:Description rdf:about="http://www.openmath.org/ontology#SignatureDictionary">
    <rdf:type rdf:resource="http://www.w3.org/2002/07/owl#Class"/>
    <rdfs:subClassOf rdf:resource="http://www.openmath.org/ontology#Dictionary"/>
    <owl:disjointWith rdf:resource="http://www.openmath.org/ontology#ContentDictionary"/>
    <rdfs:comment>An OpenMath Signature Dictionary, as described in section 4.4.  Some of the properties of signature dictionaries are defined as properties in this ontology, others are taken from Dublin Core and RDFS, with the following mapping: Name = dct:identifier</rdfs:comment>
    <rdfs:label xml:lang="en">signature dictionary</rdfs:label>
    <rdfs:isDefinedBy rdf:resource="http://www.openmath.org/ontology#"/>
  </rdf:Description>
  <rdf:Description rdf:about="http://www.openmath.org/ontology#Signature">
    <rdf:type rdf:resource="http://www.w3.org/2002/07/owl#Class"/>
    <owl:disjointWith rdf:resource="http://www.openmath.org/ontology#FormalPart"/>
    <rdfs:comment>A type signature of a symbol, as described in section 4.4</rdfs:comment>
    <owl:disjointWith rdf:resource="http://www.openmath.org/ontology#CommentedPart"/>
    <owl:disjointWith rdf:resource="http://www.openmath.org/ontology#Example"/>
    <owl:disjointWith rdf:resource="http://www.openmath.org/ontology#Status"/>
    <rdfs:isDefinedBy rdf:resource="http://www.openmath.org/ontology#"/>
    <owl:disjointWith rdf:resource="http://www.openmath.org/ontology#Composite"/>
    <rdfs:subClassOf rdf:resource="http://www.openmath.org/ontology#OpenMathConcept"/>
    <owl:disjointWith rdf:resource="http://www.openmath.org/ontology#CDBase"/>
    <rdfs:label xml:lang="en">signature</rdfs:label>
    <owl:disjointWith rdf:resource="http://www.openmath.org/ontology#Role"/>
  </rdf:Description>
  <rdf:Description rdf:nodeID="A23">
    <rdf:first rdf:resource="http://www.openmath.org/ontology#hasProperty"/>
    <rdf:rest rdf:nodeID="A28"/>
  </rdf:Description>
  <rdf:Description rdf:nodeID="A29">
    <rdf:type rdf:resource="http://www.w3.org/2002/07/owl#Restriction"/>
    <owl:onProperty rdf:resource="http://www.openmath.org/ontology#definesSymbol"/>
    <owl:minCardinality rdf:datatype="http://www.w3.org/2001/XMLSchema#nonNegativeInteger">1</owl:minCardinality>
  </rdf:Description>
  <rdf:Description rdf:about="http://www.openmath.org/ontology#base">
    <rdf:type rdf:resource="http://www.w3.org/2002/07/owl#ObjectProperty"/>
    <rdf:type rdf:resource="http://www.w3.org/2002/07/owl#FunctionalProperty"/>
    <rdfs:domain rdf:resource="http://www.openmath.org/ontology#ContentDictionary"/>
    <rdfs:range rdf:resource="http://www.openmath.org/ontology#CDBase"/>
    <rdfs:comment>The CD base URI of a content dictionary, as described in section 4.3.2</rdfs:comment>
    <rdfs:label xml:lang="en">CD base</rdfs:label>
    <rdfs:isDefinedBy rdf:resource="http://www.openmath.org/ontology#"/>
  </rdf:Description>
  <rdf:Description rdf:nodeID="A30">
    <rdf:first rdf:resource="http://www.openmath.org/ontology#Binder"/>
    <rdf:rest rdf:nodeID="A31"/>
  </rdf:Description>
  <rdf:Description rdf:nodeID="A32">
    <rdf:type rdf:resource="http://www.w3.org/2002/07/owl#Restriction"/>
    <owl:onProperty rdf:resource="http://www.openmath.org/ontology#reviewDate"/>
    <owl:allValuesFrom rdf:resource="http://www.w3.org/2001/XMLSchema#date"/>
  </rdf:Description>
  <rdf:Description rdf:nodeID="A33">
    <rdf:first rdf:resource="http://www.openmath.org/ontology#Private"/>
    <rdf:rest rdf:nodeID="A34"/>
  </rdf:Description>
  <rdf:Description rdf:nodeID="A28">
    <rdf:first rdf:resource="http://www.openmath.org/ontology#hasFormalPart"/>
    <rdf:rest rdf:nodeID="A35"/>
  </rdf:Description>
  <rdf:Description rdf:about="http://www.openmath.org/ontology#hasProperty">
    <rdf:type rdf:resource="http://www.w3.org/2002/07/owl#ObjectProperty"/>
    <rdfs:subPropertyOf rdf:resource="http://www.openmath.org/ontology#hasDirectPart"/>
    <rdfs:domain rdf:resource="http://www.openmath.org/ontology#SymbolDefinition"/>
    <rdfs:range rdf:resource="http://www.openmath.org/ontology#Property"/>
    <rdfs:comment>The relationship of a symbol definition to a CMP or FMP (OpenMath 2) or a property container that it contains</rdfs:comment>
    <rdfs:label xml:lang="en">has property</rdfs:label>
    <rdfs:isDefinedBy rdf:resource="http://www.openmath.org/ontology#"/>
  </rdf:Description>
  <rdf:Description rdf:nodeID="A18">
    <rdf:type rdf:resource="http://www.w3.org/2002/07/owl#Restriction"/>
    <owl:onProperty rdf:resource="http://www.openmath.org/ontology#major"/>
    <owl:allValuesFrom rdf:resource="http://www.w3.org/2001/XMLSchema#nonNegativeInteger"/>
  </rdf:Description>
  <rdf:Description rdf:nodeID="A14">
    <owl:unionOf rdf:nodeID="A36"/>
  </rdf:Description>
  <rdf:Description rdf:about="http://www.openmath.org/ontology#role">
    <rdf:type rdf:resource="http://www.w3.org/2002/07/owl#ObjectProperty"/>
    <rdf:type rdf:resource="http://www.w3.org/2002/07/owl#FunctionalProperty"/>
    <rdfs:domain rdf:resource="http://www.openmath.org/ontology#SymbolDefinition"/>
    <rdfs:range rdf:resource="http://www.openmath.org/ontology#Role"/>
    <rdfs:comment>The role of a symbol, as described in section 4.3.2</rdfs:comment>
    <rdfs:label xml:lang="en">role</rdfs:label>
    <rdfs:isDefinedBy rdf:resource="http://www.openmath.org/ontology#"/>
  </rdf:Description>
  <rdf:Description rdf:nodeID="A37">
    <rdf:type rdf:resource="http://www.w3.org/2002/07/owl#Restriction"/>
    <owl:onProperty rdf:resource="http://www.openmath.org/ontology#version"/>
    <owl:cardinality rdf:datatype="http://www.w3.org/2001/XMLSchema#nonNegativeInteger">1</owl:cardinality>
  </rdf:Description>
  <rdf:Description rdf:about="http://www.openmath.org/ontology#NotationDictionary">
    <rdf:type rdf:resource="http://www.w3.org/2002/07/owl#Class"/>
    <rdfs:subClassOf rdf:resource="http://www.openmath.org/ontology#Dictionary"/>
    <owl:disjointWith rdf:resource="http://www.openmath.org/ontology#ContentDictionary"/>
    <owl:disjointWith rdf:resource="http://www.openmath.org/ontology#SignatureDictionary"/>
    <rdfs:comment>This is not (yet) an official part of the OpenMath standard.  This name was conceived in analogy to “Content Dictionaries” and “Signature Dictionaries”.</rdfs:comment>
    <rdfs:label xml:lang="en">notation dictionary</rdfs:label>
    <rdfs:isDefinedBy rdf:resource="http://www.openmath.org/ontology#"/>
  </rdf:Description>
  <rdf:Description rdf:nodeID="A38">
    <rdf:first rdf:resource="http://www.openmath.org/ontology#Official"/>
    <rdf:rest rdf:nodeID="A39"/>
  </rdf:Description>
  <rdf:Description rdf:about="http://www.openmath.org/ontology#CDBase">
    <rdf:type rdf:resource="http://www.w3.org/2002/07/owl#Class"/>
    <rdfs:subClassOf rdf:resource="http://www.openmath.org/ontology#OpenMathConcept"/>
    <owl:disjointWith rdf:resource="http://www.openmath.org/ontology#Composite"/>
    <rdfs:comment>An OpenMath Content Dictionary base URI, as described in sections 2.3 and 4.2</rdfs:comment>
    <rdfs:label xml:lang="en">CD base</rdfs:label>
    <rdfs:isDefinedBy rdf:resource="http://www.openmath.org/ontology#"/>
  </rdf:Description>
  <rdf:Description rdf:about="http://www.openmath.org/ontology#Role">
    <rdf:type rdf:resource="http://www.w3.org/2002/07/owl#Class"/>
    <rdfs:subClassOf rdf:resource="http://www.openmath.org/ontology#OpenMathConcept"/>
    <owl:disjointWith rdf:resource="http://www.openmath.org/ontology#Composite"/>
    <owl:disjointWith rdf:resource="http://www.openmath.org/ontology#CDBase"/>
    <owl:disjointWith rdf:resource="http://www.openmath.org/ontology#Status"/>
    <rdfs:comment>The role of a symbol, as described in sections 2.1.4 and 4.3.2</rdfs:comment>
    <rdfs:label xml:lang="en">role</rdfs:label>
    <owl:oneOf rdf:nodeID="A30"/>
    <rdfs:isDefinedBy rdf:resource="http://www.openmath.org/ontology#"/>
  </rdf:Description>
  <rdf:Description rdf:about="http://www.openmath.org/ontology#Error">
    <rdf:type rdf:resource="http://www.openmath.org/ontology#Role"/>
    <rdfs:comment>The 'error' role of a symbol, as described in section 2.1.4</rdfs:comment>
    <rdfs:label xml:lang="en">error</rdfs:label>
    <rdfs:isDefinedBy rdf:resource="http://www.openmath.org/ontology#"/>
  </rdf:Description>
  <rdf:Description rdf:about="http://www.openmath.org/ontology#containsSignaturesFor">
    <rdf:type rdf:resource="http://www.w3.org/2002/07/owl#ObjectProperty"/>
    <rdf:type rdf:resource="http://www.w3.org/2002/07/owl#FunctionalProperty"/>
    <rdfs:domain rdf:resource="http://www.openmath.org/ontology#SignatureDictionary"/>
    <rdfs:range rdf:resource="http://www.openmath.org/ontology#ContentDictionary"/>
    <rdfs:comment>The relationship of a signature dictionary to the content dictionary whose symbols it specifies</rdfs:comment>
    <rdfs:label xml:lang="en">contains signatures for</rdfs:label>
    <rdfs:isDefinedBy rdf:resource="http://www.openmath.org/ontology#"/>
  </rdf:Description>
  <rdf:Description rdf:nodeID="A40">
    <rdf:type rdf:resource="http://www.w3.org/2002/07/owl#Restriction"/>
    <owl:onProperty rdf:resource="http://purl.org/dc/terms/identifier"/>
    <owl:allValuesFrom rdf:resource="http://www.w3.org/2001/XMLSchema#NCName"/>
  </rdf:Description>
  <rdf:Description rdf:nodeID="A39">
    <rdf:first rdf:resource="http://www.openmath.org/ontology#Experimental"/>
    <rdf:rest rdf:nodeID="A33"/>
  </rdf:Description>
  <rdf:Description rdf:about="http://www.openmath.org/ontology#definedIn">
    <rdf:type rdf:resource="http://www.w3.org/2002/07/owl#ObjectProperty"/>
    <owl:inverseOf rdf:resource="http://www.openmath.org/ontology#definesSymbol"/>
    <rdfs:comment>The relationship of a symbol definition to its enclosing content dictionary</rdfs:comment>
    <rdfs:label xml:lang="en">defined in</rdfs:label>
    <rdfs:isDefinedBy rdf:resource="http://www.openmath.org/ontology#"/>
  </rdf:Description>
  <rdf:Description rdf:nodeID="A17">
    <rdf:type rdf:resource="http://www.w3.org/2002/07/owl#Restriction"/>
    <owl:onProperty rdf:resource="http://www.openmath.org/ontology#minor"/>
    <owl:cardinality rdf:datatype="http://www.w3.org/2001/XMLSchema#nonNegativeInteger">1</owl:cardinality>
  </rdf:Description>
  <rdf:Description rdf:about="http://www.openmath.org/ontology#Application">
    <rdf:type rdf:resource="http://www.openmath.org/ontology#Role"/>
    <rdfs:comment>The 'application' role of a symbol, as described in section 2.1.4</rdfs:comment>
    <rdfs:label xml:lang="en">application</rdfs:label>
    <rdfs:isDefinedBy rdf:resource="http://www.openmath.org/ontology#"/>
  </rdf:Description>
  <rdf:Description rdf:nodeID="A36">
    <rdf:first rdf:resource="http://www.openmath.org/ontology#FormalPart"/>
    <rdf:rest rdf:nodeID="A41"/>
  </rdf:Description>
  <rdf:Description rdf:nodeID="A31">
    <rdf:first rdf:resource="http://www.openmath.org/ontology#Attribution"/>
    <rdf:rest rdf:nodeID="A42"/>
  </rdf:Description>
  <rdf:Description rdf:nodeID="A43">
    <rdf:first rdf:resource="http://www.openmath.org/ontology#ContentDictionaryGroup"/>
    <rdf:rest rdf:resource="http://www.w3.org/1999/02/22-rdf-syntax-ns#nil"/>
  </rdf:Description>
  <rdf:Description rdf:nodeID="A35">
    <rdf:first rdf:resource="http://www.openmath.org/ontology#usesSymbol"/>
    <rdf:rest rdf:nodeID="A13"/>
  </rdf:Description>
  <rdf:Description rdf:nodeID="A16">
    <rdf:type rdf:resource="http://www.w3.org/2002/07/owl#Restriction"/>
    <owl:onProperty rdf:resource="http://www.openmath.org/ontology#minor"/>
    <owl:allValuesFrom rdf:resource="http://www.w3.org/2001/XMLSchema#nonNegativeInteger"/>
  </rdf:Description>
  <rdf:Description rdf:about="http://www.openmath.org/ontology#ContentDictionaryGroup">
    <rdf:type rdf:resource="http://www.w3.org/2002/07/owl#Class"/>
    <rdfs:subClassOf rdf:resource="http://www.openmath.org/ontology#Composite"/>
    <rdfs:comment>An OpenMath CD (Content Dictionary) Group, as described in section 4.4.2.  Some of the properties of content dictionaries are defined as properties in this ontology, others are taken from Dublin Core and RDFS, with the following mapping: CDGroupName = dct:identifier, CDGroupDescription = dct:description, CDComment = rdfs:comment.</rdfs:comment>
    <rdfs:label xml:lang="en">Content Dictionary group</rdfs:label>
    <rdfs:isDefinedBy rdf:resource="http://www.openmath.org/ontology#"/>
  </rdf:Description>
  <rdf:Description rdf:about="http://www.openmath.org/ontology#containsNotationDefinition">
    <rdf:type rdf:resource="http://www.w3.org/2002/07/owl#ObjectProperty"/>
    <rdfs:subPropertyOf rdf:resource="http://www.openmath.org/ontology#hasDirectPart"/>
    <rdfs:domain rdf:resource="http://www.openmath.org/ontology#NotationDictionary"/>
    <rdfs:range rdf:resource="http://www.openmath.org/ontology#NotationDefinition"/>
    <rdfs:comment>The relationship of a notation dictionary to a notation definition it contains</rdfs:comment>
    <rdfs:label xml:lang="en">contains notation definition</rdfs:label>
    <rdfs:isDefinedBy rdf:resource="http://www.openmath.org/ontology#"/>
  </rdf:Description>
  <rdf:Description rdf:nodeID="A44">
    <rdf:type rdf:resource="http://www.w3.org/2002/07/owl#Restriction"/>
    <owl:onProperty rdf:resource="http://www.openmath.org/ontology#role"/>
    <owl:maxCardinality rdf:datatype="http://www.w3.org/2001/XMLSchema#nonNegativeInteger">1</owl:maxCardinality>
  </rdf:Description>
  <rdf:Description rdf:about="http://www.openmath.org/ontology#containsSignature">
    <rdf:type rdf:resource="http://www.w3.org/2002/07/owl#ObjectProperty"/>
    <rdfs:subPropertyOf rdf:resource="http://www.openmath.org/ontology#hasDirectPart"/>
    <rdfs:domain rdf:resource="http://www.openmath.org/ontology#SignatureDictionary"/>
    <rdfs:range rdf:resource="http://www.openmath.org/ontology#Signature"/>
    <rdfs:comment>The relationship of a signature dictionary to a type signature it contains</rdfs:comment>
    <rdfs:label xml:lang="en">contains signature</rdfs:label>
    <rdfs:isDefinedBy rdf:resource="http://www.openmath.org/ontology#"/>
  </rdf:Description>
  <rdf:Description rdf:nodeID="A45">
    <rdf:first rdf:resource="http://www.openmath.org/ontology#CommentedPart"/>
    <rdf:rest rdf:nodeID="A46"/>
  </rdf:Description>
  <rdf:Description rdf:about="http://www.openmath.org/ontology#containsNotationsFor">
    <rdf:type rdf:resource="http://www.w3.org/2002/07/owl#ObjectProperty"/>
    <rdf:type rdf:resource="http://www.w3.org/2002/07/owl#FunctionalProperty"/>
    <rdfs:domain rdf:resource="http://www.openmath.org/ontology#NotationDictionary"/>
    <rdfs:range rdf:resource="http://www.openmath.org/ontology#ContentDictionary"/>
    <rdfs:comment>The relationship of a notation dictionary to the content dictionary whose symbols it specifies</rdfs:comment>
    <rdfs:label xml:lang="en">contains notations for</rdfs:label>
    <rdfs:isDefinedBy rdf:resource="http://www.openmath.org/ontology#"/>
  </rdf:Description>
  <rdf:Description rdf:about="http://www.openmath.org/ontology#major">
    <rdf:type rdf:resource="http://www.w3.org/2002/07/owl#DatatypeProperty"/>
    <rdf:type rdf:resource="http://www.w3.org/2002/07/owl#FunctionalProperty"/>
    <rdfs:domain rdf:resource="http://www.openmath.org/ontology#Version"/>
    <rdfs:range rdf:resource="http://www.w3.org/2001/XMLSchema#nonNegativeInteger"/>
    <rdfs:comment>Major part of a version number, as described in section 4.2.2</rdfs:comment>
    <rdfs:label xml:lang="en">major part</rdfs:label>
    <rdfs:isDefinedBy rdf:resource="http://www.openmath.org/ontology#"/>
  </rdf:Description>
  <rdf:Description rdf:about="http://www.openmath.org/ontology#Composite">
    <rdf:type rdf:resource="http://www.w3.org/2002/07/owl#Class"/>
    <rdfs:subClassOf rdf:resource="http://www.openmath.org/ontology#OpenMathConcept"/>
    <rdfs:comment>The generic superclass of all concepts that can be expressed in OpenMath content/signature/notation dictionaries and that can comprise subconcepts</rdfs:comment>
    <rdfs:label xml:lang="en">composite</rdfs:label>
    <rdfs:isDefinedBy rdf:resource="http://www.openmath.org/ontology#"/>
  </rdf:Description>
  <rdf:Description rdf:about="http://purl.org/dc/terms/date">
    <rdf:type rdf:resource="http://www.w3.org/2002/07/owl#DatatypeProperty"/>
  </rdf:Description>
  <rdf:Description rdf:about="http://www.openmath.org/ontology#exemplifiedBy">
    <rdf:type rdf:resource="http://www.w3.org/2002/07/owl#ObjectProperty"/>
    <rdfs:subPropertyOf rdf:resource="http://www.openmath.org/ontology#hasDirectPart"/>
    <rdfs:domain rdf:resource="http://www.openmath.org/ontology#SymbolDefinition"/>
    <rdfs:range rdf:resource="http://www.openmath.org/ontology#Example"/>
    <rdfs:comment>The relationship of a symbol definition to an example it contains</rdfs:comment>
    <rdfs:label xml:lang="en">exemplified by</rdfs:label>
    <rdfs:isDefinedBy rdf:resource="http://www.openmath.org/ontology#"/>
  </rdf:Description>
  <rdf:Description rdf:about="http://www.openmath.org/ontology#rendersSymbol">
    <rdf:type rdf:resource="http://www.w3.org/2002/07/owl#ObjectProperty"/>
    <rdf:type rdf:resource="http://www.w3.org/2002/07/owl#FunctionalProperty"/>
    <rdfs:domain rdf:resource="http://www.openmath.org/ontology#NotationDefinition"/>
    <rdfs:range rdf:resource="http://www.openmath.org/ontology#SymbolDefinition"/>
    <rdfs:comment>The relationship of a notation definition to the symbol it renders</rdfs:comment>
    <rdfs:label xml:lang="en">renders</rdfs:label>
    <rdfs:isDefinedBy rdf:resource="http://www.openmath.org/ontology#"/>
  </rdf:Description>
  <rdf:Description rdf:nodeID="A41">
    <rdf:first rdf:resource="http://www.openmath.org/ontology#Example"/>
    <rdf:rest rdf:resource="http://www.w3.org/1999/02/22-rdf-syntax-ns#nil"/>
  </rdf:Description>
  <rdf:Description rdf:nodeID="A47">
    <rdf:first rdf:resource="http://www.openmath.org/ontology#ContentDictionary"/>
    <rdf:rest rdf:nodeID="A43"/>
  </rdf:Description>
  <rdf:Description rdf:nodeID="A42">
    <rdf:first rdf:resource="http://www.openmath.org/ontology#SemanticAttribution"/>
    <rdf:rest rdf:nodeID="A48"/>
  </rdf:Description>
  <rdf:Description rdf:about="http://www.openmath.org/ontology#version">
    <rdf:type rdf:resource="http://www.w3.org/2002/07/owl#DatatypeProperty"/>
    <rdf:type rdf:resource="http://www.w3.org/2002/07/owl#FunctionalProperty"/>
    <rdfs:domain rdf:nodeID="A27"/>
    <rdfs:range rdf:resource="http://www.openmath.org/ontology#Version"/>
    <rdfs:comment>The version of a content dictionary or content dictionary group, as described in sections 4.2.2 and 4.3.2 or 4.4.2.2, resp.</rdfs:comment>
    <rdfs:label xml:lang="en">version</rdfs:label>
    <rdfs:isDefinedBy rdf:resource="http://www.openmath.org/ontology#"/>
  </rdf:Description>
  <rdf:Description rdf:about="http://purl.org/dc/terms/title">
    <rdf:type rdf:resource="http://www.w3.org/2002/07/owl#AnnotationProperty"/>
  </rdf:Description>
  <rdf:Description rdf:nodeID="A49">
    <rdf:first rdf:resource="http://www.openmath.org/ontology#Application"/>
    <rdf:rest rdf:nodeID="A50"/>
  </rdf:Description>
  <rdf:Description rdf:nodeID="A51">
    <owl:unionOf rdf:nodeID="A45"/>
  </rdf:Description>
  <rdf:Description rdf:about="http://www.openmath.org/ontology#typesSymbol">
    <rdf:type rdf:resource="http://www.w3.org/2002/07/owl#ObjectProperty"/>
    <rdf:type rdf:resource="http://www.w3.org/2002/07/owl#FunctionalProperty"/>
    <rdfs:domain rdf:resource="http://www.openmath.org/ontology#Signature"/>
    <rdfs:range rdf:resource="http://www.openmath.org/ontology#SymbolDefinition"/>
    <rdfs:comment>The relationship of a type signature to the symbol it specifies</rdfs:comment>
    <rdfs:label xml:lang="en">types</rdfs:label>
    <rdfs:isDefinedBy rdf:resource="http://www.openmath.org/ontology#"/>
  </rdf:Description>
  <rdf:Description rdf:about="http://www.openmath.org/ontology#hasPart">
    <rdf:type rdf:resource="http://www.w3.org/2002/07/owl#TransitiveProperty"/>
    <rdf:type rdf:resource="http://www.w3.org/2002/07/owl#ObjectProperty"/>
    <rdfs:subPropertyOf rdf:resource="http://www.openmath.org/ontology#comprises"/>
    <rdfs:subPropertyOf rdf:resource="http://omdoc.org/ontology#hasPart"/>
    <rdfs:comment>This relation denotes that one concept A, directly or indirectly, logically contains another concept B, and that B is not contained by any other concept than A, as reflected by child elements in OpenMath XML documents.</rdfs:comment>
    <rdfs:label xml:lang="en">has part</rdfs:label>
    <rdfs:isDefinedBy rdf:resource="http://www.openmath.org/ontology#"/>
  </rdf:Description>
  <rdf:Description rdf:about="http://purl.org/dc/terms/contributor">
    <rdf:type rdf:resource="http://www.w3.org/2002/07/owl#AnnotationProperty"/>
  </rdf:Description>
  <rdf:Description rdf:nodeID="A46">
    <rdf:first rdf:resource="http://www.openmath.org/ontology#Example"/>
    <rdf:rest rdf:resource="http://www.w3.org/1999/02/22-rdf-syntax-ns#nil"/>
  </rdf:Description>
  <rdf:Description rdf:nodeID="A34">
    <rdf:first rdf:resource="http://www.openmath.org/ontology#Obsolete"/>
    <rdf:rest rdf:resource="http://www.w3.org/1999/02/22-rdf-syntax-ns#nil"/>
  </rdf:Description>
  <rdf:Description rdf:about="http://www.openmath.org/ontology#PragmaticSyntax">
    <rdfs:label xml:lang="en">pragmatic syntax</rdfs:label>
    <rdfs:isDefinedBy rdf:resource="http://www.openmath.org/ontology#"/>
    <owl:disjointWith rdf:resource="http://www.openmath.org/ontology#SymbolDefinition"/>
    <owl:disjointWith rdf:resource="http://www.openmath.org/ontology#ContentDictionaryGroup"/>
    <rdf:type rdf:resource="http://www.w3.org/2002/07/owl#Class"/>
    <owl:disjointWith rdf:resource="http://www.openmath.org/ontology#Dictionary"/>
    <rdfs:comment>Guidelines for using this symbol in pragmatic Content MathML</rdfs:comment>
    <owl:disjointWith rdf:resource="http://www.openmath.org/ontology#Property"/>
    <rdfs:comment>OpenMath 2+/3 transitional</rdfs:comment>
    <rdfs:subClassOf rdf:resource="http://www.openmath.org/ontology#Composite"/>
  </rdf:Description>
  <rdf:Description rdf:about="http://www.openmath.org/ontology#ContentDictionary">
    <rdfs:subClassOf rdf:nodeID="A24"/>
    <rdf:type rdf:resource="http://www.w3.org/2002/07/owl#Class"/>
    <rdfs:subClassOf rdf:nodeID="A26"/>
    <rdfs:subClassOf rdf:nodeID="A12"/>
    <rdfs:subClassOf rdf:nodeID="A32"/>
    <rdfs:comment>OpenMath 2+/3 transitional aspects: Title = dct:title</rdfs:comment>
    <rdfs:subClassOf rdf:resource="http://www.openmath.org/ontology#Dictionary"/>
    <rdfs:label xml:lang="en">Content Dictionary</rdfs:label>
    <rdfs:subClassOf rdf:nodeID="A37"/>
    <rdfs:subClassOf rdf:nodeID="A20"/>
    <rdfs:subClassOf rdf:nodeID="A4"/>
    <rdfs:isDefinedBy rdf:resource="http://www.openmath.org/ontology#"/>
    <rdfs:subClassOf rdf:nodeID="A25"/>
    <rdfs:subClassOf rdf:nodeID="A29"/>
    <rdfs:comment>An OpenMath Content Dictionary, as described in chapter 4.  Some of the properties of content dictionaries are defined as properties in this ontology, others are taken from Dublin Core and RDFS, with the following mapping: CDName = dct:identifier, Title = dct:title, Description = dct:description, CDDate = dct:date, CDComment = rdfs:comment.</rdfs:comment>
    <rdfs:subClassOf rdf:nodeID="A40"/>
  </rdf:Description>
  <rdf:Description rdf:nodeID="A22">
    <rdf:first rdf:resource="http://www.openmath.org/ontology#definesSymbol"/>
    <rdf:rest rdf:nodeID="A0"/>
  </rdf:Description>
  <rdf:Description rdf:nodeID="A9">
    <owl:unionOf rdf:nodeID="A47"/>
  </rdf:Description>
  <rdf:Description rdf:about="http://www.openmath.org/ontology#Status">
    <rdf:type rdf:resource="http://www.w3.org/2002/07/owl#Class"/>
    <rdfs:subClassOf rdf:resource="http://www.openmath.org/ontology#OpenMathConcept"/>
    <owl:oneOf rdf:nodeID="A38"/>
    <owl:disjointWith rdf:resource="http://www.openmath.org/ontology#Composite"/>
    <owl:disjointWith rdf:resource="http://www.openmath.org/ontology#CDBase"/>
    <rdfs:comment>The status of a CD, as described in sections 4.2.1 and 4.3.2</rdfs:comment>
    <rdfs:label xml:lang="en">status</rdfs:label>
    <rdfs:isDefinedBy rdf:resource="http://www.openmath.org/ontology#"/>
  </rdf:Description>
  <rdf:Description rdf:about="http://www.openmath.org/ontology#hasText">
    <rdf:type rdf:resource="http://www.w3.org/2002/07/owl#DatatypeProperty"/>
    <rdfs:domain rdf:nodeID="A51"/>
    <rdfs:range rdf:resource="http://www.w3.org/2000/01/rdf-schema#Literal"/>
    <rdfs:comment>The text of a property (usually an informal one)</rdfs:comment>
    <rdfs:label xml:lang="en">text</rdfs:label>
    <rdfs:isDefinedBy rdf:resource="http://www.openmath.org/ontology#"/>
  </rdf:Description>
  <rdf:Description rdf:nodeID="A50">
    <rdf:first rdf:resource="http://www.openmath.org/ontology#Constant"/>
    <rdf:rest rdf:resource="http://www.w3.org/1999/02/22-rdf-syntax-ns#nil"/>
  </rdf:Description>
  <rdf:Description rdf:nodeID="A48">
    <rdf:first rdf:resource="http://www.openmath.org/ontology#Error"/>
    <rdf:rest rdf:nodeID="A49"/>
  </rdf:Description>
  <rdf:Description rdf:about="http://www.openmath.org/ontology#Official">
    <rdf:type rdf:resource="http://www.openmath.org/ontology#Status"/>
    <rdfs:comment>The 'official' status of a CD, as described in section 4.2.1</rdfs:comment>
    <rdfs:label xml:lang="en">official</rdfs:label>
    <rdfs:isDefinedBy rdf:resource="http://www.openmath.org/ontology#"/>
  </rdf:Description>
  <rdf:Description rdf:about="http://www.openmath.org/ontology#CommentedPart">
    <rdf:type rdf:resource="http://www.w3.org/2002/07/owl#Class"/>
    <rdfs:subClassOf rdf:resource="http://www.openmath.org/ontology#OpenMathConcept"/>
    <owl:disjointWith rdf:resource="http://www.openmath.org/ontology#Composite"/>
    <owl:disjointWith rdf:resource="http://www.openmath.org/ontology#CDBase"/>
    <owl:disjointWith rdf:resource="http://www.openmath.org/ontology#Status"/>
    <owl:disjointWith rdf:resource="http://www.openmath.org/ontology#Role"/>
    <rdfs:comment>A commented part of a mathematical property (CMP) of a symbol, as described in sections 4.2 and 4.3</rdfs:comment>
    <rdfs:label xml:lang="en">commented part</rdfs:label>
    <rdfs:isDefinedBy rdf:resource="http://www.openmath.org/ontology#"/>
  </rdf:Description>
</rdf:RDF>
